Update Isabelle snapshots
Except RISC-V duopod, which doesn't seem to build for me at the moment

snapshots/isabelle/aarch64/Aarch64_lemmas.thy
@@ -1,11 +1,11 @@
 theory Aarch64_lemmas
   imports
-    Sail.Sail_values_lemmas
-    Sail.State_lemmas
+    Sail.Sail2_values_lemmas
+    Sail.Sail2_state_lemmas
     Aarch64
 begin
 
-abbreviation "liftS \<equiv> liftState (get_regval, set_regval)"
+abbreviation liftS ("\<lbrakk>_\<rbrakk>\<^sub>S") where "liftS \<equiv> liftState (get_regval, set_regval)"
 
 lemmas register_defs = get_regval_def set_regval_def APDAKeyHi_EL1_ref_def APDAKeyLo_EL1_ref_def
   APDBKeyHi_EL1_ref_def APDBKeyLo_EL1_ref_def APGAKeyHi_EL1_ref_def APGAKeyLo_EL1_ref_def
@@ -80,996 +80,1009 @@ proof -
   then show ?thesis by (auto simp: vector_of_regval_def regval_of_vector_def)
 qed
 
-lemma liftS_read_reg_APDAKeyHi_EL1[simp]:
-  "liftS (read_reg APDAKeyHi_EL1_ref) = readS (APDAKeyHi_EL1 \<circ> regstate)"
+lemma option_of_rv_rv_of_option[simp]:
+  assumes "\<And>v. of_rv (rv_of v) = Some v"
+  shows "option_of_regval of_rv (regval_of_option rv_of v) = Some v"
+  using assms by (cases v) (auto simp: option_of_regval_def regval_of_option_def)
+
+lemma list_of_rv_rv_of_list[simp]:
+  assumes "\<And>v. of_rv (rv_of v) = Some v"
+  shows "list_of_regval of_rv (regval_of_list rv_of v) = Some v"
+proof -
+  from assms have "of_rv \<circ> rv_of = Some" by auto
+  with assms show ?thesis by (induction v) (auto simp: list_of_regval_def regval_of_list_def)
+qed
+
+lemma liftS_read_reg_APDAKeyHi_EL1[liftState_simp]:
+  "\<lbrakk>read_reg APDAKeyHi_EL1_ref\<rbrakk>\<^sub>S = readS (APDAKeyHi_EL1 \<circ> regstate)"
   by (auto simp: liftState_read_reg_readS register_defs)
 
-lemma liftS_write_reg_APDAKeyHi_EL1[simp]:
-  "liftS (write_reg APDAKeyHi_EL1_ref v) = updateS (regstate_update (APDAKeyHi_EL1_update (\<lambda>_. v)))"
+lemma liftS_write_reg_APDAKeyHi_EL1[liftState_simp]:
+  "\<lbrakk>write_reg APDAKeyHi_EL1_ref v\<rbrakk>\<^sub>S = updateS (regstate_update (APDAKeyHi_EL1_update (\<lambda>_. v)))"
   by (auto simp: liftState_write_reg_updateS register_defs)
 
-lemma liftS_read_reg_APDAKeyLo_EL1[simp]:
-  "liftS (read_reg APDAKeyLo_EL1_ref) = readS (APDAKeyLo_EL1 \<circ> regstate)"
+lemma liftS_read_reg_APDAKeyLo_EL1[liftState_simp]:
+  "\<lbrakk>read_reg APDAKeyLo_EL1_ref\<rbrakk>\<^sub>S = readS (APDAKeyLo_EL1 \<circ> regstate)"
   by (auto simp: liftState_read_reg_readS register_defs)
 
-lemma liftS_write_reg_APDAKeyLo_EL1[simp]:
-  "liftS (write_reg APDAKeyLo_EL1_ref v) = updateS (regstate_update (APDAKeyLo_EL1_update (\<lambda>_. v)))"
+lemma liftS_write_reg_APDAKeyLo_EL1[liftState_simp]:
+  "\<lbrakk>write_reg APDAKeyLo_EL1_ref v\<rbrakk>\<^sub>S = updateS (regstate_update (APDAKeyLo_EL1_update (\<lambda>_. v)))"
   by (auto simp: liftState_write_reg_updateS register_defs)
 
-lemma liftS_read_reg_APDBKeyHi_EL1[simp]:
-  "liftS (read_reg APDBKeyHi_EL1_ref) = readS (APDBKeyHi_EL1 \<circ> regstate)"
+lemma liftS_read_reg_APDBKeyHi_EL1[liftState_simp]:
+  "\<lbrakk>read_reg APDBKeyHi_EL1_ref\<rbrakk>\<^sub>S = readS (APDBKeyHi_EL1 \<circ> regstate)"
   by (auto simp: liftState_read_reg_readS register_defs)
 
-lemma liftS_write_reg_APDBKeyHi_EL1[simp]:
-  "liftS (write_reg APDBKeyHi_EL1_ref v) = updateS (regstate_update (APDBKeyHi_EL1_update (\<lambda>_. v)))"
+lemma liftS_write_reg_APDBKeyHi_EL1[liftState_simp]:
+  "\<lbrakk>write_reg APDBKeyHi_EL1_ref v\<rbrakk>\<^sub>S = updateS (regstate_update (APDBKeyHi_EL1_update (\<lambda>_. v)))"
   by (auto simp: liftState_write_reg_updateS register_defs)
 
-lemma liftS_read_reg_APDBKeyLo_EL1[simp]:
-  "liftS (read_reg APDBKeyLo_EL1_ref) = readS (APDBKeyLo_EL1 \<circ> regstate)"
+lemma liftS_read_reg_APDBKeyLo_EL1[liftState_simp]:
+  "\<lbrakk>read_reg APDBKeyLo_EL1_ref\<rbrakk>\<^sub>S = readS (APDBKeyLo_EL1 \<circ> regstate)"
   by (auto simp: liftState_read_reg_readS register_defs)
 
-lemma liftS_write_reg_APDBKeyLo_EL1[simp]:
-  "liftS (write_reg APDBKeyLo_EL1_ref v) = updateS (regstate_update (APDBKeyLo_EL1_update (\<lambda>_. v)))"
+lemma liftS_write_reg_APDBKeyLo_EL1[liftState_simp]:
+  "\<lbrakk>write_reg APDBKeyLo_EL1_ref v\<rbrakk>\<^sub>S = updateS (regstate_update (APDBKeyLo_EL1_update (\<lambda>_. v)))"
   by (auto simp: liftState_write_reg_updateS register_defs)
 
-lemma liftS_read_reg_APGAKeyHi_EL1[simp]:
-  "liftS (read_reg APGAKeyHi_EL1_ref) = readS (APGAKeyHi_EL1 \<circ> regstate)"
+lemma liftS_read_reg_APGAKeyHi_EL1[liftState_simp]:
+  "\<lbrakk>read_reg APGAKeyHi_EL1_ref\<rbrakk>\<^sub>S = readS (APGAKeyHi_EL1 \<circ> regstate)"
   by (auto simp: liftState_read_reg_readS register_defs)
 
-lemma liftS_write_reg_APGAKeyHi_EL1[simp]:
-  "liftS (write_reg APGAKeyHi_EL1_ref v) = updateS (regstate_update (APGAKeyHi_EL1_update (\<lambda>_. v)))"
+lemma liftS_write_reg_APGAKeyHi_EL1[liftState_simp]:
+  "\<lbrakk>write_reg APGAKeyHi_EL1_ref v\<rbrakk>\<^sub>S = updateS (regstate_update (APGAKeyHi_EL1_update (\<lambda>_. v)))"
   by (auto simp: liftState_write_reg_updateS register_defs)
 
-lemma liftS_read_reg_APGAKeyLo_EL1[simp]:
-  "liftS (read_reg APGAKeyLo_EL1_ref) = readS (APGAKeyLo_EL1 \<circ> regstate)"
+lemma liftS_read_reg_APGAKeyLo_EL1[liftState_simp]:
+  "\<lbrakk>read_reg APGAKeyLo_EL1_ref\<rbrakk>\<^sub>S = readS (APGAKeyLo_EL1 \<circ> regstate)"
   by (auto simp: liftState_read_reg_readS register_defs)
 
-lemma liftS_write_reg_APGAKeyLo_EL1[simp]:
-  "liftS (write_reg APGAKeyLo_EL1_ref v) = updateS (regstate_update (APGAKeyLo_EL1_update (\<lambda>_. v)))"
+lemma liftS_write_reg_APGAKeyLo_EL1[liftState_simp]:
+  "\<lbrakk>write_reg APGAKeyLo_EL1_ref v\<rbrakk>\<^sub>S = updateS (regstate_update (APGAKeyLo_EL1_update (\<lambda>_. v)))"
   by (auto simp: liftState_write_reg_updateS register_defs)
 
-lemma liftS_read_reg_APIAKeyHi_EL1[simp]:
-  "liftS (read_reg APIAKeyHi_EL1_ref) = readS (APIAKeyHi_EL1 \<circ> regstate)"
+lemma liftS_read_reg_APIAKeyHi_EL1[liftState_simp]:
+  "\<lbrakk>read_reg APIAKeyHi_EL1_ref\<rbrakk>\<^sub>S = readS (APIAKeyHi_EL1 \<circ> regstate)"
   by (auto simp: liftState_read_reg_readS register_defs)
 
-lemma liftS_write_reg_APIAKeyHi_EL1[simp]:
-  "liftS (write_reg APIAKeyHi_EL1_ref v) = updateS (regstate_update (APIAKeyHi_EL1_update (\<lambda>_. v)))"
+lemma liftS_write_reg_APIAKeyHi_EL1[liftState_simp]:
+  "\<lbrakk>write_reg APIAKeyHi_EL1_ref v\<rbrakk>\<^sub>S = updateS (regstate_update (APIAKeyHi_EL1_update (\<lambda>_. v)))"
   by (auto simp: liftState_write_reg_updateS register_defs)
 
-lemma liftS_read_reg_APIAKeyLo_EL1[simp]:
-  "liftS (read_reg APIAKeyLo_EL1_ref) = readS (APIAKeyLo_EL1 \<circ> regstate)"
+lemma liftS_read_reg_APIAKeyLo_EL1[liftState_simp]:
+  "\<lbrakk>read_reg APIAKeyLo_EL1_ref\<rbrakk>\<^sub>S = readS (APIAKeyLo_EL1 \<circ> regstate)"
   by (auto simp: liftState_read_reg_readS register_defs)
 
-lemma liftS_write_reg_APIAKeyLo_EL1[simp]:
-  "liftS (write_reg APIAKeyLo_EL1_ref v) = updateS (regstate_update (APIAKeyLo_EL1_update (\<lambda>_. v)))"
+lemma liftS_write_reg_APIAKeyLo_EL1[liftState_simp]:
+  "\<lbrakk>write_reg APIAKeyLo_EL1_ref v\<rbrakk>\<^sub>S = updateS (regstate_update (APIAKeyLo_EL1_update (\<lambda>_. v)))"
   by (auto simp: liftState_write_reg_updateS register_defs)
 
-lemma liftS_read_reg_APIBKeyHi_EL1[simp]:
-  "liftS (read_reg APIBKeyHi_EL1_ref) = readS (APIBKeyHi_EL1 \<circ> regstate)"
+lemma liftS_read_reg_APIBKeyHi_EL1[liftState_simp]:
+  "\<lbrakk>read_reg APIBKeyHi_EL1_ref\<rbrakk>\<^sub>S = readS (APIBKeyHi_EL1 \<circ> regstate)"
   by (auto simp: liftState_read_reg_readS register_defs)
 
-lemma liftS_write_reg_APIBKeyHi_EL1[simp]:
-  "liftS (write_reg APIBKeyHi_EL1_ref v) = updateS (regstate_update (APIBKeyHi_EL1_update (\<lambda>_. v)))"
+lemma liftS_write_reg_APIBKeyHi_EL1[liftState_simp]:
+  "\<lbrakk>write_reg APIBKeyHi_EL1_ref v\<rbrakk>\<^sub>S = updateS (regstate_update (APIBKeyHi_EL1_update (\<lambda>_. v)))"
   by (auto simp: liftState_write_reg_updateS register_defs)
 
-lemma liftS_read_reg_APIBKeyLo_EL1[simp]:
-  "liftS (read_reg APIBKeyLo_EL1_ref) = readS (APIBKeyLo_EL1 \<circ> regstate)"
+lemma liftS_read_reg_APIBKeyLo_EL1[liftState_simp]:
+  "\<lbrakk>read_reg APIBKeyLo_EL1_ref\<rbrakk>\<^sub>S = readS (APIBKeyLo_EL1 \<circ> regstate)"
   by (auto simp: liftState_read_reg_readS register_defs)
 
-lemma liftS_write_reg_APIBKeyLo_EL1[simp]:
-  "liftS (write_reg APIBKeyLo_EL1_ref v) = updateS (regstate_update (APIBKeyLo_EL1_update (\<lambda>_. v)))"
+lemma liftS_write_reg_APIBKeyLo_EL1[liftState_simp]:
+  "\<lbrakk>write_reg APIBKeyLo_EL1_ref v\<rbrakk>\<^sub>S = updateS (regstate_update (APIBKeyLo_EL1_update (\<lambda>_. v)))"
   by (auto simp: liftState_write_reg_updateS register_defs)
 
-lemma liftS_read_reg_CONTEXTIDR_EL1[simp]:
-  "liftS (read_reg CONTEXTIDR_EL1_ref) = readS (CONTEXTIDR_EL1 \<circ> regstate)"
+lemma liftS_read_reg_CONTEXTIDR_EL1[liftState_simp]:
+  "\<lbrakk>read_reg CONTEXTIDR_EL1_ref\<rbrakk>\<^sub>S = readS (CONTEXTIDR_EL1 \<circ> regstate)"
   by (auto simp: liftState_read_reg_readS register_defs)
 
-lemma liftS_write_reg_CONTEXTIDR_EL1[simp]:
-  "liftS (write_reg CONTEXTIDR_EL1_ref v) = updateS (regstate_update (CONTEXTIDR_EL1_update (\<lambda>_. v)))"
+lemma liftS_write_reg_CONTEXTIDR_EL1[liftState_simp]:
+  "\<lbrakk>write_reg CONTEXTIDR_EL1_ref v\<rbrakk>\<^sub>S = updateS (regstate_update (CONTEXTIDR_EL1_update (\<lambda>_. v)))"
   by (auto simp: liftState_write_reg_updateS register_defs)
 
-lemma liftS_read_reg_CONTEXTIDR_EL2[simp]:
-  "liftS (read_reg CONTEXTIDR_EL2_ref) = readS (CONTEXTIDR_EL2 \<circ> regstate)"
+lemma liftS_read_reg_CONTEXTIDR_EL2[liftState_simp]:
+  "\<lbrakk>read_reg CONTEXTIDR_EL2_ref\<rbrakk>\<^sub>S = readS (CONTEXTIDR_EL2 \<circ> regstate)"
   by (auto simp: liftState_read_reg_readS register_defs)
 
-lemma liftS_write_reg_CONTEXTIDR_EL2[simp]:
-  "liftS (write_reg CONTEXTIDR_EL2_ref v) = updateS (regstate_update (CONTEXTIDR_EL2_update (\<lambda>_. v)))"
+lemma liftS_write_reg_CONTEXTIDR_EL2[liftState_simp]:
+  "\<lbrakk>write_reg CONTEXTIDR_EL2_ref v\<rbrakk>\<^sub>S = updateS (regstate_update (CONTEXTIDR_EL2_update (\<lambda>_. v)))"
   by (auto simp: liftState_write_reg_updateS register_defs)
 
-lemma liftS_read_reg_CPACR_EL1[simp]:
-  "liftS (read_reg CPACR_EL1_ref) = readS (CPACR_EL1 \<circ> regstate)"
+lemma liftS_read_reg_CPACR_EL1[liftState_simp]:
+  "\<lbrakk>read_reg CPACR_EL1_ref\<rbrakk>\<^sub>S = readS (CPACR_EL1 \<circ> regstate)"
   by (auto simp: liftState_read_reg_readS register_defs)
 
-lemma liftS_write_reg_CPACR_EL1[simp]:
-  "liftS (write_reg CPACR_EL1_ref v) = updateS (regstate_update (CPACR_EL1_update (\<lambda>_. v)))"
+lemma liftS_write_reg_CPACR_EL1[liftState_simp]:
+  "\<lbrakk>write_reg CPACR_EL1_ref v\<rbrakk>\<^sub>S = updateS (regstate_update (CPACR_EL1_update (\<lambda>_. v)))"
   by (auto simp: liftState_write_reg_updateS register_defs)
 
-lemma liftS_read_reg_CPTR_EL2[simp]:
-  "liftS (read_reg CPTR_EL2_ref) = readS (CPTR_EL2 \<circ> regstate)"
+lemma liftS_read_reg_CPTR_EL2[liftState_simp]:
+  "\<lbrakk>read_reg CPTR_EL2_ref\<rbrakk>\<^sub>S = readS (CPTR_EL2 \<circ> regstate)"
   by (auto simp: liftState_read_reg_readS register_defs)
 
-lemma liftS_write_reg_CPTR_EL2[simp]:
-  "liftS (write_reg CPTR_EL2_ref v) = updateS (regstate_update (CPTR_EL2_update (\<lambda>_. v)))"
+lemma liftS_write_reg_CPTR_EL2[liftState_simp]:
+  "\<lbrakk>write_reg CPTR_EL2_ref v\<rbrakk>\<^sub>S = updateS (regstate_update (CPTR_EL2_update (\<lambda>_. v)))"
   by (auto simp: liftState_write_reg_updateS register_defs)
 
-lemma liftS_read_reg_CPTR_EL3[simp]:
-  "liftS (read_reg CPTR_EL3_ref) = readS (CPTR_EL3 \<circ> regstate)"
+lemma liftS_read_reg_CPTR_EL3[liftState_simp]:
+  "\<lbrakk>read_reg CPTR_EL3_ref\<rbrakk>\<^sub>S = readS (CPTR_EL3 \<circ> regstate)"
   by (auto simp: liftState_read_reg_readS register_defs)
 
-lemma liftS_write_reg_CPTR_EL3[simp]:
-  "liftS (write_reg CPTR_EL3_ref v) = updateS (regstate_update (CPTR_EL3_update (\<lambda>_. v)))"
+lemma liftS_write_reg_CPTR_EL3[liftState_simp]:
+  "\<lbrakk>write_reg CPTR_EL3_ref v\<rbrakk>\<^sub>S = updateS (regstate_update (CPTR_EL3_update (\<lambda>_. v)))"
   by (auto simp: liftState_write_reg_updateS register_defs)
 
-lemma liftS_read_reg_DBGBCR_EL1[simp]:
-  "liftS (read_reg DBGBCR_EL1_ref) = readS (DBGBCR_EL1 \<circ> regstate)"
+lemma liftS_read_reg_DBGBCR_EL1[liftState_simp]:
+  "\<lbrakk>read_reg DBGBCR_EL1_ref\<rbrakk>\<^sub>S = readS (DBGBCR_EL1 \<circ> regstate)"
   by (auto simp: liftState_read_reg_readS register_defs)
 
-lemma liftS_write_reg_DBGBCR_EL1[simp]:
-  "liftS (write_reg DBGBCR_EL1_ref v) = updateS (regstate_update (DBGBCR_EL1_update (\<lambda>_. v)))"
+lemma liftS_write_reg_DBGBCR_EL1[liftState_simp]:
+  "\<lbrakk>write_reg DBGBCR_EL1_ref v\<rbrakk>\<^sub>S = updateS (regstate_update (DBGBCR_EL1_update (\<lambda>_. v)))"
   by (auto simp: liftState_write_reg_updateS register_defs)
 
-lemma liftS_read_reg_DBGBVR_EL1[simp]:
-  "liftS (read_reg DBGBVR_EL1_ref) = readS (DBGBVR_EL1 \<circ> regstate)"
+lemma liftS_read_reg_DBGBVR_EL1[liftState_simp]:
+  "\<lbrakk>read_reg DBGBVR_EL1_ref\<rbrakk>\<^sub>S = readS (DBGBVR_EL1 \<circ> regstate)"
   by (auto simp: liftState_read_reg_readS register_defs)
 
-lemma liftS_write_reg_DBGBVR_EL1[simp]:
-  "liftS (write_reg DBGBVR_EL1_ref v) = updateS (regstate_update (DBGBVR_EL1_update (\<lambda>_. v)))"
+lemma liftS_write_reg_DBGBVR_EL1[liftState_simp]:
+  "\<lbrakk>write_reg DBGBVR_EL1_ref v\<rbrakk>\<^sub>S = updateS (regstate_update (DBGBVR_EL1_update (\<lambda>_. v)))"
   by (auto simp: liftState_write_reg_updateS register_defs)
 
-lemma liftS_read_reg_DBGEN[simp]:
-  "liftS (read_reg DBGEN_ref) = readS (DBGEN \<circ> regstate)"
+lemma liftS_read_reg_DBGEN[liftState_simp]:
+  "\<lbrakk>read_reg DBGEN_ref\<rbrakk>\<^sub>S = readS (DBGEN \<circ> regstate)"
   by (auto simp: liftState_read_reg_readS register_defs)
 
-lemma liftS_write_reg_DBGEN[simp]:
-  "liftS (write_reg DBGEN_ref v) = updateS (regstate_update (DBGEN_update (\<lambda>_. v)))"
+lemma liftS_write_reg_DBGEN[liftState_simp]:
+  "\<lbrakk>write_reg DBGEN_ref v\<rbrakk>\<^sub>S = updateS (regstate_update (DBGEN_update (\<lambda>_. v)))"
   by (auto simp: liftState_write_reg_updateS register_defs)
 
-lemma liftS_read_reg_DBGOSDLR[simp]:
-  "liftS (read_reg DBGOSDLR_ref) = readS (DBGOSDLR \<circ> regstate)"
+lemma liftS_read_reg_DBGOSDLR[liftState_simp]:
+  "\<lbrakk>read_reg DBGOSDLR_ref\<rbrakk>\<^sub>S = readS (DBGOSDLR \<circ> regstate)"
   by (auto simp: liftState_read_reg_readS register_defs)
 
-lemma liftS_write_reg_DBGOSDLR[simp]:
-  "liftS (write_reg DBGOSDLR_ref v) = updateS (regstate_update (DBGOSDLR_update (\<lambda>_. v)))"
+lemma liftS_write_reg_DBGOSDLR[liftState_simp]:
+  "\<lbrakk>write_reg DBGOSDLR_ref v\<rbrakk>\<^sub>S = updateS (regstate_update (DBGOSDLR_update (\<lambda>_. v)))"
   by (auto simp: liftState_write_reg_updateS register_defs)
 
-lemma liftS_read_reg_DBGOSLSR[simp]:
-  "liftS (read_reg DBGOSLSR_ref) = readS (DBGOSLSR \<circ> regstate)"
+lemma liftS_read_reg_DBGOSLSR[liftState_simp]:
+  "\<lbrakk>read_reg DBGOSLSR_ref\<rbrakk>\<^sub>S = readS (DBGOSLSR \<circ> regstate)"
   by (auto simp: liftState_read_reg_readS register_defs)
 
-lemma liftS_write_reg_DBGOSLSR[simp]:
-  "liftS (write_reg DBGOSLSR_ref v) = updateS (regstate_update (DBGOSLSR_update (\<lambda>_. v)))"
+lemma liftS_write_reg_DBGOSLSR[liftState_simp]:
+  "\<lbrakk>write_reg DBGOSLSR_ref v\<rbrakk>\<^sub>S = updateS (regstate_update (DBGOSLSR_update (\<lambda>_. v)))"
   by (auto simp: liftState_write_reg_updateS register_defs)
 
-lemma liftS_read_reg_DBGPRCR[simp]:
-  "liftS (read_reg DBGPRCR_ref) = readS (DBGPRCR \<circ> regstate)"
+lemma liftS_read_reg_DBGPRCR[liftState_simp]:
+  "\<lbrakk>read_reg DBGPRCR_ref\<rbrakk>\<^sub>S = readS (DBGPRCR \<circ> regstate)"
   by (auto simp: liftState_read_reg_readS register_defs)
 
-lemma liftS_write_reg_DBGPRCR[simp]:
-  "liftS (write_reg DBGPRCR_ref v) = updateS (regstate_update (DBGPRCR_update (\<lambda>_. v)))"
+lemma liftS_write_reg_DBGPRCR[liftState_simp]:
+  "\<lbrakk>write_reg DBGPRCR_ref v\<rbrakk>\<^sub>S = updateS (regstate_update (DBGPRCR_update (\<lambda>_. v)))"
   by (auto simp: liftState_write_reg_updateS register_defs)
 
-lemma liftS_read_reg_DBGPRCR_EL1[simp]:
-  "liftS (read_reg DBGPRCR_EL1_ref) = readS (DBGPRCR_EL1 \<circ> regstate)"
+lemma liftS_read_reg_DBGPRCR_EL1[liftState_simp]:
+  "\<lbrakk>read_reg DBGPRCR_EL1_ref\<rbrakk>\<^sub>S = readS (DBGPRCR_EL1 \<circ> regstate)"
   by (auto simp: liftState_read_reg_readS register_defs)
 
-lemma liftS_write_reg_DBGPRCR_EL1[simp]:
-  "liftS (write_reg DBGPRCR_EL1_ref v) = updateS (regstate_update (DBGPRCR_EL1_update (\<lambda>_. v)))"
+lemma liftS_write_reg_DBGPRCR_EL1[liftState_simp]:
+  "\<lbrakk>write_reg DBGPRCR_EL1_ref v\<rbrakk>\<^sub>S = updateS (regstate_update (DBGPRCR_EL1_update (\<lambda>_. v)))"
   by (auto simp: liftState_write_reg_updateS register_defs)
 
-lemma liftS_read_reg_DBGWCR_EL1[simp]:
-  "liftS (read_reg DBGWCR_EL1_ref) = readS (DBGWCR_EL1 \<circ> regstate)"
+lemma liftS_read_reg_DBGWCR_EL1[liftState_simp]:
+  "\<lbrakk>read_reg DBGWCR_EL1_ref\<rbrakk>\<^sub>S = readS (DBGWCR_EL1 \<circ> regstate)"
   by (auto simp: liftState_read_reg_readS register_defs)
 
-lemma liftS_write_reg_DBGWCR_EL1[simp]:
-  "liftS (write_reg DBGWCR_EL1_ref v) = updateS (regstate_update (DBGWCR_EL1_update (\<lambda>_. v)))"
+lemma liftS_write_reg_DBGWCR_EL1[liftState_simp]:
+  "\<lbrakk>write_reg DBGWCR_EL1_ref v\<rbrakk>\<^sub>S = updateS (regstate_update (DBGWCR_EL1_update (\<lambda>_. v)))"
   by (auto simp: liftState_write_reg_updateS register_defs)
 
-lemma liftS_read_reg_DBGWVR_EL1[simp]:
-  "liftS (read_reg DBGWVR_EL1_ref) = readS (DBGWVR_EL1 \<circ> regstate)"
+lemma liftS_read_reg_DBGWVR_EL1[liftState_simp]:
+  "\<lbrakk>read_reg DBGWVR_EL1_ref\<rbrakk>\<^sub>S = readS (DBGWVR_EL1 \<circ> regstate)"
   by (auto simp: liftState_read_reg_readS register_defs)
 
-lemma liftS_write_reg_DBGWVR_EL1[simp]:
-  "liftS (write_reg DBGWVR_EL1_ref v) = updateS (regstate_update (DBGWVR_EL1_update (\<lambda>_. v)))"
+lemma liftS_write_reg_DBGWVR_EL1[liftState_simp]:
+  "\<lbrakk>write_reg DBGWVR_EL1_ref v\<rbrakk>\<^sub>S = updateS (regstate_update (DBGWVR_EL1_update (\<lambda>_. v)))"
   by (auto simp: liftState_write_reg_updateS register_defs)
 
-lemma liftS_read_reg_DLR[simp]:
-  "liftS (read_reg DLR_ref) = readS (DLR \<circ> regstate)"
+lemma liftS_read_reg_DLR[liftState_simp]:
+  "\<lbrakk>read_reg DLR_ref\<rbrakk>\<^sub>S = readS (DLR \<circ> regstate)"
   by (auto simp: liftState_read_reg_readS register_defs)
 
-lemma liftS_write_reg_DLR[simp]:
-  "liftS (write_reg DLR_ref v) = updateS (regstate_update (DLR_update (\<lambda>_. v)))"
+lemma liftS_write_reg_DLR[liftState_simp]:
+  "\<lbrakk>write_reg DLR_ref v\<rbrakk>\<^sub>S = updateS (regstate_update (DLR_update (\<lambda>_. v)))"
   by (auto simp: liftState_write_reg_updateS register_defs)
 
-lemma liftS_read_reg_DLR_EL0[simp]:
-  "liftS (read_reg DLR_EL0_ref) = readS (DLR_EL0 \<circ> regstate)"
+lemma liftS_read_reg_DLR_EL0[liftState_simp]:
+  "\<lbrakk>read_reg DLR_EL0_ref\<rbrakk>\<^sub>S = readS (DLR_EL0 \<circ> regstate)"
   by (auto simp: liftState_read_reg_readS register_defs)
 
-lemma liftS_write_reg_DLR_EL0[simp]:
-  "liftS (write_reg DLR_EL0_ref v) = updateS (regstate_update (DLR_EL0_update (\<lambda>_. v)))"
+lemma liftS_write_reg_DLR_EL0[liftState_simp]:
+  "\<lbrakk>write_reg DLR_EL0_ref v\<rbrakk>\<^sub>S = updateS (regstate_update (DLR_EL0_update (\<lambda>_. v)))"
   by (auto simp: liftState_write_reg_updateS register_defs)
 
-lemma liftS_read_reg_DSPSR[simp]:
-  "liftS (read_reg DSPSR_ref) = readS (DSPSR \<circ> regstate)"
+lemma liftS_read_reg_DSPSR[liftState_simp]:
+  "\<lbrakk>read_reg DSPSR_ref\<rbrakk>\<^sub>S = readS (DSPSR \<circ> regstate)"
   by (auto simp: liftState_read_reg_readS register_defs)
 
-lemma liftS_write_reg_DSPSR[simp]:
-  "liftS (write_reg DSPSR_ref v) = updateS (regstate_update (DSPSR_update (\<lambda>_. v)))"
+lemma liftS_write_reg_DSPSR[liftState_simp]:
+  "\<lbrakk>write_reg DSPSR_ref v\<rbrakk>\<^sub>S = updateS (regstate_update (DSPSR_update (\<lambda>_. v)))"
   by (auto simp: liftState_write_reg_updateS register_defs)
 
-lemma liftS_read_reg_DSPSR_EL0[simp]:
-  "liftS (read_reg DSPSR_EL0_ref) = readS (DSPSR_EL0 \<circ> regstate)"
+lemma liftS_read_reg_DSPSR_EL0[liftState_simp]:
+  "\<lbrakk>read_reg DSPSR_EL0_ref\<rbrakk>\<^sub>S = readS (DSPSR_EL0 \<circ> regstate)"
   by (auto simp: liftState_read_reg_readS register_defs)
 
-lemma liftS_write_reg_DSPSR_EL0[simp]:
-  "liftS (write_reg DSPSR_EL0_ref v) = updateS (regstate_update (DSPSR_EL0_update (\<lambda>_. v)))"
+lemma liftS_write_reg_DSPSR_EL0[liftState_simp]:
+  "\<lbrakk>write_reg DSPSR_EL0_ref v\<rbrakk>\<^sub>S = updateS (regstate_update (DSPSR_EL0_update (\<lambda>_. v)))"
   by (auto simp: liftState_write_reg_updateS register_defs)
 
-lemma liftS_read_reg_EDSCR[simp]:
-  "liftS (read_reg EDSCR_ref) = readS (EDSCR \<circ> regstate)"
+lemma liftS_read_reg_EDSCR[liftState_simp]:
+  "\<lbrakk>read_reg EDSCR_ref\<rbrakk>\<^sub>S = readS (EDSCR \<circ> regstate)"
   by (auto simp: liftState_read_reg_readS register_defs)
 
-lemma liftS_write_reg_EDSCR[simp]:
-  "liftS (write_reg EDSCR_ref v) = updateS (regstate_update (EDSCR_update (\<lambda>_. v)))"
+lemma liftS_write_reg_EDSCR[liftState_simp]:
+  "\<lbrakk>write_reg EDSCR_ref v\<rbrakk>\<^sub>S = updateS (regstate_update (EDSCR_update (\<lambda>_. v)))"
   by (auto simp: liftState_write_reg_updateS register_defs)
 
-lemma liftS_read_reg_ELR_EL1[simp]:
-  "liftS (read_reg ELR_EL1_ref) = readS (ELR_EL1 \<circ> regstate)"
+lemma liftS_read_reg_ELR_EL1[liftState_simp]:
+  "\<lbrakk>read_reg ELR_EL1_ref\<rbrakk>\<^sub>S = readS (ELR_EL1 \<circ> regstate)"
   by (auto simp: liftState_read_reg_readS register_defs)
 
-lemma liftS_write_reg_ELR_EL1[simp]:
-  "liftS (write_reg ELR_EL1_ref v) = updateS (regstate_update (ELR_EL1_update (\<lambda>_. v)))"
+lemma liftS_write_reg_ELR_EL1[liftState_simp]:
+  "\<lbrakk>write_reg ELR_EL1_ref v\<rbrakk>\<^sub>S = updateS (regstate_update (ELR_EL1_update (\<lambda>_. v)))"
   by (auto simp: liftState_write_reg_updateS register_defs)
 
-lemma liftS_read_reg_ELR_EL2[simp]:
-  "liftS (read_reg ELR_EL2_ref) = readS (ELR_EL2 \<circ> regstate)"
+lemma liftS_read_reg_ELR_EL2[liftState_simp]:
+  "\<lbrakk>read_reg ELR_EL2_ref\<rbrakk>\<^sub>S = readS (ELR_EL2 \<circ> regstate)"
   by (auto simp: liftState_read_reg_readS register_defs)
 
-lemma liftS_write_reg_ELR_EL2[simp]:
-  "liftS (write_reg ELR_EL2_ref v) = updateS (regstate_update (ELR_EL2_update (\<lambda>_. v)))"
+lemma liftS_write_reg_ELR_EL2[liftState_simp]:
+  "\<lbrakk>write_reg ELR_EL2_ref v\<rbrakk>\<^sub>S = updateS (regstate_update (ELR_EL2_update (\<lambda>_. v)))"
   by (auto simp: liftState_write_reg_updateS register_defs)
 
-lemma liftS_read_reg_ELR_EL3[simp]:
-  "liftS (read_reg ELR_EL3_ref) = readS (ELR_EL3 \<circ> regstate)"
+lemma liftS_read_reg_ELR_EL3[liftState_simp]:
+  "\<lbrakk>read_reg ELR_EL3_ref\<rbrakk>\<^sub>S = readS (ELR_EL3 \<circ> regstate)"
   by (auto simp: liftState_read_reg_readS register_defs)
 
-lemma liftS_write_reg_ELR_EL3[simp]:
-  "liftS (write_reg ELR_EL3_ref v) = updateS (regstate_update (ELR_EL3_update (\<lambda>_. v)))"
+lemma liftS_write_reg_ELR_EL3[liftState_simp]:
+  "\<lbrakk>write_reg ELR_EL3_ref v\<rbrakk>\<^sub>S = updateS (regstate_update (ELR_EL3_update (\<lambda>_. v)))"
   by (auto simp: liftState_write_reg_updateS register_defs)
 
-lemma liftS_read_reg_ELR_hyp[simp]:
-  "liftS (read_reg ELR_hyp_ref) = readS (ELR_hyp \<circ> regstate)"
+lemma liftS_read_reg_ELR_hyp[liftState_simp]:
+  "\<lbrakk>read_reg ELR_hyp_ref\<rbrakk>\<^sub>S = readS (ELR_hyp \<circ> regstate)"
   by (auto simp: liftState_read_reg_readS register_defs)
 
-lemma liftS_write_reg_ELR_hyp[simp]:
-  "liftS (write_reg ELR_hyp_ref v) = updateS (regstate_update (ELR_hyp_update (\<lambda>_. v)))"
+lemma liftS_write_reg_ELR_hyp[liftState_simp]:
+  "\<lbrakk>write_reg ELR_hyp_ref v\<rbrakk>\<^sub>S = updateS (regstate_update (ELR_hyp_update (\<lambda>_. v)))"
   by (auto simp: liftState_write_reg_updateS register_defs)
 
-lemma liftS_read_reg_ESR_EL1[simp]:
-  "liftS (read_reg ESR_EL1_ref) = readS (ESR_EL1 \<circ> regstate)"
+lemma liftS_read_reg_ESR_EL1[liftState_simp]:
+  "\<lbrakk>read_reg ESR_EL1_ref\<rbrakk>\<^sub>S = readS (ESR_EL1 \<circ> regstate)"
   by (auto simp: liftState_read_reg_readS register_defs)
 
-lemma liftS_write_reg_ESR_EL1[simp]:
-  "liftS (write_reg ESR_EL1_ref v) = updateS (regstate_update (ESR_EL1_update (\<lambda>_. v)))"
+lemma liftS_write_reg_ESR_EL1[liftState_simp]:
+  "\<lbrakk>write_reg ESR_EL1_ref v\<rbrakk>\<^sub>S = updateS (regstate_update (ESR_EL1_update (\<lambda>_. v)))"
   by (auto simp: liftState_write_reg_updateS register_defs)
 
-lemma liftS_read_reg_ESR_EL2[simp]:
-  "liftS (read_reg ESR_EL2_ref) = readS (ESR_EL2 \<circ> regstate)"
+lemma liftS_read_reg_ESR_EL2[liftState_simp]:
+  "\<lbrakk>read_reg ESR_EL2_ref\<rbrakk>\<^sub>S = readS (ESR_EL2 \<circ> regstate)"
   by (auto simp: liftState_read_reg_readS register_defs)
 
-lemma liftS_write_reg_ESR_EL2[simp]:
-  "liftS (write_reg ESR_EL2_ref v) = updateS (regstate_update (ESR_EL2_update (\<lambda>_. v)))"
+lemma liftS_write_reg_ESR_EL2[liftState_simp]:
+  "\<lbrakk>write_reg ESR_EL2_ref v\<rbrakk>\<^sub>S = updateS (regstate_update (ESR_EL2_update (\<lambda>_. v)))"
   by (auto simp: liftState_write_reg_updateS register_defs)
 
-lemma liftS_read_reg_ESR_EL3[simp]:
-  "liftS (read_reg ESR_EL3_ref) = readS (ESR_EL3 \<circ> regstate)"
+lemma liftS_read_reg_ESR_EL3[liftState_simp]:
+  "\<lbrakk>read_reg ESR_EL3_ref\<rbrakk>\<^sub>S = readS (ESR_EL3 \<circ> regstate)"
   by (auto simp: liftState_read_reg_readS register_defs)
 
-lemma liftS_write_reg_ESR_EL3[simp]:
-  "liftS (write_reg ESR_EL3_ref v) = updateS (regstate_update (ESR_EL3_update (\<lambda>_. v)))"
+lemma liftS_write_reg_ESR_EL3[liftState_simp]:
+  "\<lbrakk>write_reg ESR_EL3_ref v\<rbrakk>\<^sub>S = updateS (regstate_update (ESR_EL3_update (\<lambda>_. v)))"
   by (auto simp: liftState_write_reg_updateS register_defs)
 
-lemma liftS_read_reg_EventRegister[simp]:
-  "liftS (read_reg EventRegister_ref) = readS (EventRegister \<circ> regstate)"
+lemma liftS_read_reg_EventRegister[liftState_simp]:
+  "\<lbrakk>read_reg EventRegister_ref\<rbrakk>\<^sub>S = readS (EventRegister \<circ> regstate)"
   by (auto simp: liftState_read_reg_readS register_defs)
 
-lemma liftS_write_reg_EventRegister[simp]:
-  "liftS (write_reg EventRegister_ref v) = updateS (regstate_update (EventRegister_update (\<lambda>_. v)))"
+lemma liftS_write_reg_EventRegister[liftState_simp]:
+  "\<lbrakk>write_reg EventRegister_ref v\<rbrakk>\<^sub>S = updateS (regstate_update (EventRegister_update (\<lambda>_. v)))"
   by (auto simp: liftState_write_reg_updateS register_defs)
 
-lemma liftS_read_reg_FAR_EL1[simp]:
-  "liftS (read_reg FAR_EL1_ref) = readS (FAR_EL1 \<circ> regstate)"
+lemma liftS_read_reg_FAR_EL1[liftState_simp]:
+  "\<lbrakk>read_reg FAR_EL1_ref\<rbrakk>\<^sub>S = readS (FAR_EL1 \<circ> regstate)"
   by (auto simp: liftState_read_reg_readS register_defs)
 
-lemma liftS_write_reg_FAR_EL1[simp]:
-  "liftS (write_reg FAR_EL1_ref v) = updateS (regstate_update (FAR_EL1_update (\<lambda>_. v)))"
+lemma liftS_write_reg_FAR_EL1[liftState_simp]:
+  "\<lbrakk>write_reg FAR_EL1_ref v\<rbrakk>\<^sub>S = updateS (regstate_update (FAR_EL1_update (\<lambda>_. v)))"
   by (auto simp: liftState_write_reg_updateS register_defs)
 
-lemma liftS_read_reg_FAR_EL2[simp]:
-  "liftS (read_reg FAR_EL2_ref) = readS (FAR_EL2 \<circ> regstate)"
+lemma liftS_read_reg_FAR_EL2[liftState_simp]:
+  "\<lbrakk>read_reg FAR_EL2_ref\<rbrakk>\<^sub>S = readS (FAR_EL2 \<circ> regstate)"
   by (auto simp: liftState_read_reg_readS register_defs)
 
-lemma liftS_write_reg_FAR_EL2[simp]:
-  "liftS (write_reg FAR_EL2_ref v) = updateS (regstate_update (FAR_EL2_update (\<lambda>_. v)))"
+lemma liftS_write_reg_FAR_EL2[liftState_simp]:
+  "\<lbrakk>write_reg FAR_EL2_ref v\<rbrakk>\<^sub>S = updateS (regstate_update (FAR_EL2_update (\<lambda>_. v)))"
   by (auto simp: liftState_write_reg_updateS register_defs)
 
-lemma liftS_read_reg_FAR_EL3[simp]:
-  "liftS (read_reg FAR_EL3_ref) = readS (FAR_EL3 \<circ> regstate)"
+lemma liftS_read_reg_FAR_EL3[liftState_simp]:
+  "\<lbrakk>read_reg FAR_EL3_ref\<rbrakk>\<^sub>S = readS (FAR_EL3 \<circ> regstate)"
   by (auto simp: liftState_read_reg_readS register_defs)
 
-lemma liftS_write_reg_FAR_EL3[simp]:
-  "liftS (write_reg FAR_EL3_ref v) = updateS (regstate_update (FAR_EL3_update (\<lambda>_. v)))"
+lemma liftS_write_reg_FAR_EL3[liftState_simp]:
+  "\<lbrakk>write_reg FAR_EL3_ref v\<rbrakk>\<^sub>S = updateS (regstate_update (FAR_EL3_update (\<lambda>_. v)))"
   by (auto simp: liftState_write_reg_updateS register_defs)
 
-lemma liftS_read_reg_FPCR[simp]:
-  "liftS (read_reg FPCR_ref) = readS (FPCR \<circ> regstate)"
+lemma liftS_read_reg_FPCR[liftState_simp]:
+  "\<lbrakk>read_reg FPCR_ref\<rbrakk>\<^sub>S = readS (FPCR \<circ> regstate)"
   by (auto simp: liftState_read_reg_readS register_defs)
 
-lemma liftS_write_reg_FPCR[simp]:
-  "liftS (write_reg FPCR_ref v) = updateS (regstate_update (FPCR_update (\<lambda>_. v)))"
+lemma liftS_write_reg_FPCR[liftState_simp]:
+  "\<lbrakk>write_reg FPCR_ref v\<rbrakk>\<^sub>S = updateS (regstate_update (FPCR_update (\<lambda>_. v)))"
   by (auto simp: liftState_write_reg_updateS register_defs)
 
-lemma liftS_read_reg_FPEXC[simp]:
-  "liftS (read_reg FPEXC_ref) = readS (FPEXC \<circ> regstate)"
+lemma liftS_read_reg_FPEXC[liftState_simp]:
+  "\<lbrakk>read_reg FPEXC_ref\<rbrakk>\<^sub>S = readS (FPEXC \<circ> regstate)"
   by (auto simp: liftState_read_reg_readS register_defs)
 
-lemma liftS_write_reg_FPEXC[simp]:
-  "liftS (write_reg FPEXC_ref v) = updateS (regstate_update (FPEXC_update (\<lambda>_. v)))"
+lemma liftS_write_reg_FPEXC[liftState_simp]:
+  "\<lbrakk>write_reg FPEXC_ref v\<rbrakk>\<^sub>S = updateS (regstate_update (FPEXC_update (\<lambda>_. v)))"
   by (auto simp: liftState_write_reg_updateS register_defs)
 
-lemma liftS_read_reg_FPSCR[simp]:
-  "liftS (read_reg FPSCR_ref) = readS (FPSCR \<circ> regstate)"
+lemma liftS_read_reg_FPSCR[liftState_simp]:
+  "\<lbrakk>read_reg FPSCR_ref\<rbrakk>\<^sub>S = readS (FPSCR \<circ> regstate)"
   by (auto simp: liftState_read_reg_readS register_defs)
 
-lemma liftS_write_reg_FPSCR[simp]:
-  "liftS (write_reg FPSCR_ref v) = updateS (regstate_update (FPSCR_update (\<lambda>_. v)))"
+lemma liftS_write_reg_FPSCR[liftState_simp]:
+  "\<lbrakk>write_reg FPSCR_ref v\<rbrakk>\<^sub>S = updateS (regstate_update (FPSCR_update (\<lambda>_. v)))"
   by (auto simp: liftState_write_reg_updateS register_defs)
 
-lemma liftS_read_reg_FPSR[simp]:
-  "liftS (read_reg FPSR_ref) = readS (FPSR \<circ> regstate)"
+lemma liftS_read_reg_FPSR[liftState_simp]:
+  "\<lbrakk>read_reg FPSR_ref\<rbrakk>\<^sub>S = readS (FPSR \<circ> regstate)"
   by (auto simp: liftState_read_reg_readS register_defs)
 
-lemma liftS_write_reg_FPSR[simp]:
-  "liftS (write_reg FPSR_ref v) = updateS (regstate_update (FPSR_update (\<lambda>_. v)))"
+lemma liftS_write_reg_FPSR[liftState_simp]:
+  "\<lbrakk>write_reg FPSR_ref v\<rbrakk>\<^sub>S = updateS (regstate_update (FPSR_update (\<lambda>_. v)))"
   by (auto simp: liftState_write_reg_updateS register_defs)
 
-lemma liftS_read_reg_HCR[simp]:
-  "liftS (read_reg HCR_ref) = readS (HCR \<circ> regstate)"
+lemma liftS_read_reg_HCR[liftState_simp]:
+  "\<lbrakk>read_reg HCR_ref\<rbrakk>\<^sub>S = readS (HCR \<circ> regstate)"
   by (auto simp: liftState_read_reg_readS register_defs)
 
-lemma liftS_write_reg_HCR[simp]:
-  "liftS (write_reg HCR_ref v) = updateS (regstate_update (HCR_update (\<lambda>_. v)))"
+lemma liftS_write_reg_HCR[liftState_simp]:
+  "\<lbrakk>write_reg HCR_ref v\<rbrakk>\<^sub>S = updateS (regstate_update (HCR_update (\<lambda>_. v)))"
   by (auto simp: liftState_write_reg_updateS register_defs)
 
-lemma liftS_read_reg_HCR2[simp]:
-  "liftS (read_reg HCR2_ref) = readS (HCR2 \<circ> regstate)"
+lemma liftS_read_reg_HCR2[liftState_simp]:
+  "\<lbrakk>read_reg HCR2_ref\<rbrakk>\<^sub>S = readS (HCR2 \<circ> regstate)"
   by (auto simp: liftState_read_reg_readS register_defs)
 
-lemma liftS_write_reg_HCR2[simp]:
-  "liftS (write_reg HCR2_ref v) = updateS (regstate_update (HCR2_update (\<lambda>_. v)))"
+lemma liftS_write_reg_HCR2[liftState_simp]:
+  "\<lbrakk>write_reg HCR2_ref v\<rbrakk>\<^sub>S = updateS (regstate_update (HCR2_update (\<lambda>_. v)))"
   by (auto simp: liftState_write_reg_updateS register_defs)
 
-lemma liftS_read_reg_HCR_EL2[simp]:
-  "liftS (read_reg HCR_EL2_ref) = readS (HCR_EL2 \<circ> regstate)"
+lemma liftS_read_reg_HCR_EL2[liftState_simp]:
+  "\<lbrakk>read_reg HCR_EL2_ref\<rbrakk>\<^sub>S = readS (HCR_EL2 \<circ> regstate)"
   by (auto simp: liftState_read_reg_readS register_defs)
 
-lemma liftS_write_reg_HCR_EL2[simp]:
-  "liftS (write_reg HCR_EL2_ref v) = updateS (regstate_update (HCR_EL2_update (\<lambda>_. v)))"
+lemma liftS_write_reg_HCR_EL2[liftState_simp]:
+  "\<lbrakk>write_reg HCR_EL2_ref v\<rbrakk>\<^sub>S = updateS (regstate_update (HCR_EL2_update (\<lambda>_. v)))"
   by (auto simp: liftState_write_reg_updateS register_defs)
 
-lemma liftS_read_reg_HDCR[simp]:
-  "liftS (read_reg HDCR_ref) = readS (HDCR \<circ> regstate)"
+lemma liftS_read_reg_HDCR[liftState_simp]:
+  "\<lbrakk>read_reg HDCR_ref\<rbrakk>\<^sub>S = readS (HDCR \<circ> regstate)"
   by (auto simp: liftState_read_reg_readS register_defs)
 
-lemma liftS_write_reg_HDCR[simp]:
-  "liftS (write_reg HDCR_ref v) = updateS (regstate_update (HDCR_update (\<lambda>_. v)))"
+lemma liftS_write_reg_HDCR[liftState_simp]:
+  "\<lbrakk>write_reg HDCR_ref v\<rbrakk>\<^sub>S = updateS (regstate_update (HDCR_update (\<lambda>_. v)))"
   by (auto simp: liftState_write_reg_updateS register_defs)
 
-lemma liftS_read_reg_HDFAR[simp]:
-  "liftS (read_reg HDFAR_ref) = readS (HDFAR \<circ> regstate)"
+lemma liftS_read_reg_HDFAR[liftState_simp]:
+  "\<lbrakk>read_reg HDFAR_ref\<rbrakk>\<^sub>S = readS (HDFAR \<circ> regstate)"
   by (auto simp: liftState_read_reg_readS register_defs)
 
-lemma liftS_write_reg_HDFAR[simp]:
-  "liftS (write_reg HDFAR_ref v) = updateS (regstate_update (HDFAR_update (\<lambda>_. v)))"
+lemma liftS_write_reg_HDFAR[liftState_simp]:
+  "\<lbrakk>write_reg HDFAR_ref v\<rbrakk>\<^sub>S = updateS (regstate_update (HDFAR_update (\<lambda>_. v)))"
   by (auto simp: liftState_write_reg_updateS register_defs)
 
-lemma liftS_read_reg_HIFAR[simp]:
-  "liftS (read_reg HIFAR_ref) = readS (HIFAR \<circ> regstate)"
+lemma liftS_read_reg_HIFAR[liftState_simp]:
+  "\<lbrakk>read_reg HIFAR_ref\<rbrakk>\<^sub>S = readS (HIFAR \<circ> regstate)"
   by (auto simp: liftState_read_reg_readS register_defs)
 
-lemma liftS_write_reg_HIFAR[simp]:
-  "liftS (write_reg HIFAR_ref v) = updateS (regstate_update (HIFAR_update (\<lambda>_. v)))"
+lemma liftS_write_reg_HIFAR[liftState_simp]:
+  "\<lbrakk>write_reg HIFAR_ref v\<rbrakk>\<^sub>S = updateS (regstate_update (HIFAR_update (\<lambda>_. v)))"
   by (auto simp: liftState_write_reg_updateS register_defs)
 
-lemma liftS_read_reg_HPFAR[simp]:
-  "liftS (read_reg HPFAR_ref) = readS (HPFAR \<circ> regstate)"
+lemma liftS_read_reg_HPFAR[liftState_simp]:
+  "\<lbrakk>read_reg HPFAR_ref\<rbrakk>\<^sub>S = readS (HPFAR \<circ> regstate)"
   by (auto simp: liftState_read_reg_readS register_defs)
 
-lemma liftS_write_reg_HPFAR[simp]:
-  "liftS (write_reg HPFAR_ref v) = updateS (regstate_update (HPFAR_update (\<lambda>_. v)))"
+lemma liftS_write_reg_HPFAR[liftState_simp]:
+  "\<lbrakk>write_reg HPFAR_ref v\<rbrakk>\<^sub>S = updateS (regstate_update (HPFAR_update (\<lambda>_. v)))"
   by (auto simp: liftState_write_reg_updateS register_defs)
 
-lemma liftS_read_reg_HPFAR_EL2[simp]:
-  "liftS (read_reg HPFAR_EL2_ref) = readS (HPFAR_EL2 \<circ> regstate)"
+lemma liftS_read_reg_HPFAR_EL2[liftState_simp]:
+  "\<lbrakk>read_reg HPFAR_EL2_ref\<rbrakk>\<^sub>S = readS (HPFAR_EL2 \<circ> regstate)"
   by (auto simp: liftState_read_reg_readS register_defs)
 
-lemma liftS_write_reg_HPFAR_EL2[simp]:
-  "liftS (write_reg HPFAR_EL2_ref v) = updateS (regstate_update (HPFAR_EL2_update (\<lambda>_. v)))"
+lemma liftS_write_reg_HPFAR_EL2[liftState_simp]:
+  "\<lbrakk>write_reg HPFAR_EL2_ref v\<rbrakk>\<^sub>S = updateS (regstate_update (HPFAR_EL2_update (\<lambda>_. v)))"
   by (auto simp: liftState_write_reg_updateS register_defs)
 
-lemma liftS_read_reg_HSCTLR[simp]:
-  "liftS (read_reg HSCTLR_ref) = readS (HSCTLR \<circ> regstate)"
+lemma liftS_read_reg_HSCTLR[liftState_simp]:
+  "\<lbrakk>read_reg HSCTLR_ref\<rbrakk>\<^sub>S = readS (HSCTLR \<circ> regstate)"
   by (auto simp: liftState_read_reg_readS register_defs)
 
-lemma liftS_write_reg_HSCTLR[simp]:
-  "liftS (write_reg HSCTLR_ref v) = updateS (regstate_update (HSCTLR_update (\<lambda>_. v)))"
+lemma liftS_write_reg_HSCTLR[liftState_simp]:
+  "\<lbrakk>write_reg HSCTLR_ref v\<rbrakk>\<^sub>S = updateS (regstate_update (HSCTLR_update (\<lambda>_. v)))"
   by (auto simp: liftState_write_reg_updateS register_defs)
 
-lemma liftS_read_reg_HSR[simp]:
-  "liftS (read_reg HSR_ref) = readS (HSR \<circ> regstate)"
+lemma liftS_read_reg_HSR[liftState_simp]:
+  "\<lbrakk>read_reg HSR_ref\<rbrakk>\<^sub>S = readS (HSR \<circ> regstate)"
   by (auto simp: liftState_read_reg_readS register_defs)
 
-lemma liftS_write_reg_HSR[simp]:
-  "liftS (write_reg HSR_ref v) = updateS (regstate_update (HSR_update (\<lambda>_. v)))"
+lemma liftS_write_reg_HSR[liftState_simp]:
+  "\<lbrakk>write_reg HSR_ref v\<rbrakk>\<^sub>S = updateS (regstate_update (HSR_update (\<lambda>_. v)))"
   by (auto simp: liftState_write_reg_updateS register_defs)
 
-lemma liftS_read_reg_HVBAR[simp]:
-  "liftS (read_reg HVBAR_ref) = readS (HVBAR \<circ> regstate)"
+lemma liftS_read_reg_HVBAR[liftState_simp]:
+  "\<lbrakk>read_reg HVBAR_ref\<rbrakk>\<^sub>S = readS (HVBAR \<circ> regstate)"
   by (auto simp: liftState_read_reg_readS register_defs)
 
-lemma liftS_write_reg_HVBAR[simp]:
-  "liftS (write_reg HVBAR_ref v) = updateS (regstate_update (HVBAR_update (\<lambda>_. v)))"
+lemma liftS_write_reg_HVBAR[liftState_simp]:
+  "\<lbrakk>write_reg HVBAR_ref v\<rbrakk>\<^sub>S = updateS (regstate_update (HVBAR_update (\<lambda>_. v)))"
   by (auto simp: liftState_write_reg_updateS register_defs)
 
-lemma liftS_read_reg_ID_AA64DFR0_EL1[simp]:
-  "liftS (read_reg ID_AA64DFR0_EL1_ref) = readS (ID_AA64DFR0_EL1 \<circ> regstate)"
+lemma liftS_read_reg_ID_AA64DFR0_EL1[liftState_simp]:
+  "\<lbrakk>read_reg ID_AA64DFR0_EL1_ref\<rbrakk>\<^sub>S = readS (ID_AA64DFR0_EL1 \<circ> regstate)"
   by (auto simp: liftState_read_reg_readS register_defs)
 
-lemma liftS_write_reg_ID_AA64DFR0_EL1[simp]:
-  "liftS (write_reg ID_AA64DFR0_EL1_ref v) = updateS (regstate_update (ID_AA64DFR0_EL1_update (\<lambda>_. v)))"
+lemma liftS_write_reg_ID_AA64DFR0_EL1[liftState_simp]:
+  "\<lbrakk>write_reg ID_AA64DFR0_EL1_ref v\<rbrakk>\<^sub>S = updateS (regstate_update (ID_AA64DFR0_EL1_update (\<lambda>_. v)))"
   by (auto simp: liftState_write_reg_updateS register_defs)
 
-lemma liftS_read_reg_LR_mon[simp]:
-  "liftS (read_reg LR_mon_ref) = readS (LR_mon \<circ> regstate)"
+lemma liftS_read_reg_LR_mon[liftState_simp]:
+  "\<lbrakk>read_reg LR_mon_ref\<rbrakk>\<^sub>S = readS (LR_mon \<circ> regstate)"
   by (auto simp: liftState_read_reg_readS register_defs)
 
-lemma liftS_write_reg_LR_mon[simp]:
-  "liftS (write_reg LR_mon_ref v) = updateS (regstate_update (LR_mon_update (\<lambda>_. v)))"
+lemma liftS_write_reg_LR_mon[liftState_simp]:
+  "\<lbrakk>write_reg LR_mon_ref v\<rbrakk>\<^sub>S = updateS (regstate_update (LR_mon_update (\<lambda>_. v)))"
   by (auto simp: liftState_write_reg_updateS register_defs)
 
-lemma liftS_read_reg_MAIR_EL1[simp]:
-  "liftS (read_reg MAIR_EL1_ref) = readS (MAIR_EL1 \<circ> regstate)"
+lemma liftS_read_reg_MAIR_EL1[liftState_simp]:
+  "\<lbrakk>read_reg MAIR_EL1_ref\<rbrakk>\<^sub>S = readS (MAIR_EL1 \<circ> regstate)"
   by (auto simp: liftState_read_reg_readS register_defs)
 
-lemma liftS_write_reg_MAIR_EL1[simp]:
-  "liftS (write_reg MAIR_EL1_ref v) = updateS (regstate_update (MAIR_EL1_update (\<lambda>_. v)))"
+lemma liftS_write_reg_MAIR_EL1[liftState_simp]:
+  "\<lbrakk>write_reg MAIR_EL1_ref v\<rbrakk>\<^sub>S = updateS (regstate_update (MAIR_EL1_update (\<lambda>_. v)))"
   by (auto simp: liftState_write_reg_updateS register_defs)
 
-lemma liftS_read_reg_MAIR_EL2[simp]:
-  "liftS (read_reg MAIR_EL2_ref) = readS (MAIR_EL2 \<circ> regstate)"
+lemma liftS_read_reg_MAIR_EL2[liftState_simp]:
+  "\<lbrakk>read_reg MAIR_EL2_ref\<rbrakk>\<^sub>S = readS (MAIR_EL2 \<circ> regstate)"
   by (auto simp: liftState_read_reg_readS register_defs)
 
-lemma liftS_write_reg_MAIR_EL2[simp]:
-  "liftS (write_reg MAIR_EL2_ref v) = updateS (regstate_update (MAIR_EL2_update (\<lambda>_. v)))"
+lemma liftS_write_reg_MAIR_EL2[liftState_simp]:
+  "\<lbrakk>write_reg MAIR_EL2_ref v\<rbrakk>\<^sub>S = updateS (regstate_update (MAIR_EL2_update (\<lambda>_. v)))"
   by (auto simp: liftState_write_reg_updateS register_defs)
 
-lemma liftS_read_reg_MAIR_EL3[simp]:
-  "liftS (read_reg MAIR_EL3_ref) = readS (MAIR_EL3 \<circ> regstate)"
+lemma liftS_read_reg_MAIR_EL3[liftState_simp]:
+  "\<lbrakk>read_reg MAIR_EL3_ref\<rbrakk>\<^sub>S = readS (MAIR_EL3 \<circ> regstate)"
   by (auto simp: liftState_read_reg_readS register_defs)
 
-lemma liftS_write_reg_MAIR_EL3[simp]:
-  "liftS (write_reg MAIR_EL3_ref v) = updateS (regstate_update (MAIR_EL3_update (\<lambda>_. v)))"
+lemma liftS_write_reg_MAIR_EL3[liftState_simp]:
+  "\<lbrakk>write_reg MAIR_EL3_ref v\<rbrakk>\<^sub>S = updateS (regstate_update (MAIR_EL3_update (\<lambda>_. v)))"
   by (auto simp: liftState_write_reg_updateS register_defs)
 
-lemma liftS_read_reg_MDCR_EL2[simp]:
-  "liftS (read_reg MDCR_EL2_ref) = readS (MDCR_EL2 \<circ> regstate)"
+lemma liftS_read_reg_MDCR_EL2[liftState_simp]:
+  "\<lbrakk>read_reg MDCR_EL2_ref\<rbrakk>\<^sub>S = readS (MDCR_EL2 \<circ> regstate)"
   by (auto simp: liftState_read_reg_readS register_defs)
 
-lemma liftS_write_reg_MDCR_EL2[simp]:
-  "liftS (write_reg MDCR_EL2_ref v) = updateS (regstate_update (MDCR_EL2_update (\<lambda>_. v)))"
+lemma liftS_write_reg_MDCR_EL2[liftState_simp]:
+  "\<lbrakk>write_reg MDCR_EL2_ref v\<rbrakk>\<^sub>S = updateS (regstate_update (MDCR_EL2_update (\<lambda>_. v)))"
   by (auto simp: liftState_write_reg_updateS register_defs)
 
-lemma liftS_read_reg_MDCR_EL3[simp]:
-  "liftS (read_reg MDCR_EL3_ref) = readS (MDCR_EL3 \<circ> regstate)"
+lemma liftS_read_reg_MDCR_EL3[liftState_simp]:
+  "\<lbrakk>read_reg MDCR_EL3_ref\<rbrakk>\<^sub>S = readS (MDCR_EL3 \<circ> regstate)"
   by (auto simp: liftState_read_reg_readS register_defs)
 
-lemma liftS_write_reg_MDCR_EL3[simp]:
-  "liftS (write_reg MDCR_EL3_ref v) = updateS (regstate_update (MDCR_EL3_update (\<lambda>_. v)))"
+lemma liftS_write_reg_MDCR_EL3[liftState_simp]:
+  "\<lbrakk>write_reg MDCR_EL3_ref v\<rbrakk>\<^sub>S = updateS (regstate_update (MDCR_EL3_update (\<lambda>_. v)))"
   by (auto simp: liftState_write_reg_updateS register_defs)
 
-lemma liftS_read_reg_MDSCR_EL1[simp]:
-  "liftS (read_reg MDSCR_EL1_ref) = readS (MDSCR_EL1 \<circ> regstate)"
+lemma liftS_read_reg_MDSCR_EL1[liftState_simp]:
+  "\<lbrakk>read_reg MDSCR_EL1_ref\<rbrakk>\<^sub>S = readS (MDSCR_EL1 \<circ> regstate)"
   by (auto simp: liftState_read_reg_readS register_defs)
 
-lemma liftS_write_reg_MDSCR_EL1[simp]:
-  "liftS (write_reg MDSCR_EL1_ref v) = updateS (regstate_update (MDSCR_EL1_update (\<lambda>_. v)))"
+lemma liftS_write_reg_MDSCR_EL1[liftState_simp]:
+  "\<lbrakk>write_reg MDSCR_EL1_ref v\<rbrakk>\<^sub>S = updateS (regstate_update (MDSCR_EL1_update (\<lambda>_. v)))"
   by (auto simp: liftState_write_reg_updateS register_defs)
 
-lemma liftS_read_reg_OSDLR_EL1[simp]:
-  "liftS (read_reg OSDLR_EL1_ref) = readS (OSDLR_EL1 \<circ> regstate)"
+lemma liftS_read_reg_OSDLR_EL1[liftState_simp]:
+  "\<lbrakk>read_reg OSDLR_EL1_ref\<rbrakk>\<^sub>S = readS (OSDLR_EL1 \<circ> regstate)"
   by (auto simp: liftState_read_reg_readS register_defs)
 
-lemma liftS_write_reg_OSDLR_EL1[simp]:
-  "liftS (write_reg OSDLR_EL1_ref v) = updateS (regstate_update (OSDLR_EL1_update (\<lambda>_. v)))"
+lemma liftS_write_reg_OSDLR_EL1[liftState_simp]:
+  "\<lbrakk>write_reg OSDLR_EL1_ref v\<rbrakk>\<^sub>S = updateS (regstate_update (OSDLR_EL1_update (\<lambda>_. v)))"
   by (auto simp: liftState_write_reg_updateS register_defs)
 
-lemma liftS_read_reg_OSLSR_EL1[simp]:
-  "liftS (read_reg OSLSR_EL1_ref) = readS (OSLSR_EL1 \<circ> regstate)"
+lemma liftS_read_reg_OSLSR_EL1[liftState_simp]:
+  "\<lbrakk>read_reg OSLSR_EL1_ref\<rbrakk>\<^sub>S = readS (OSLSR_EL1 \<circ> regstate)"
   by (auto simp: liftState_read_reg_readS register_defs)
 
-lemma liftS_write_reg_OSLSR_EL1[simp]:
-  "liftS (write_reg OSLSR_EL1_ref v) = updateS (regstate_update (OSLSR_EL1_update (\<lambda>_. v)))"
+lemma liftS_write_reg_OSLSR_EL1[liftState_simp]:
+  "\<lbrakk>write_reg OSLSR_EL1_ref v\<rbrakk>\<^sub>S = updateS (regstate_update (OSLSR_EL1_update (\<lambda>_. v)))"
   by (auto simp: liftState_write_reg_updateS register_defs)
 
-lemma liftS_read_reg_PSTATE[simp]:
-  "liftS (read_reg PSTATE_ref) = readS (PSTATE \<circ> regstate)"
+lemma liftS_read_reg_PSTATE[liftState_simp]:
+  "\<lbrakk>read_reg PSTATE_ref\<rbrakk>\<^sub>S = readS (PSTATE \<circ> regstate)"
   by (auto simp: liftState_read_reg_readS register_defs)
 
-lemma liftS_write_reg_PSTATE[simp]:
-  "liftS (write_reg PSTATE_ref v) = updateS (regstate_update (PSTATE_update (\<lambda>_. v)))"
+lemma liftS_write_reg_PSTATE[liftState_simp]:
+  "\<lbrakk>write_reg PSTATE_ref v\<rbrakk>\<^sub>S = updateS (regstate_update (PSTATE_update (\<lambda>_. v)))"
   by (auto simp: liftState_write_reg_updateS register_defs)
 
-lemma liftS_read_reg_RC[simp]:
-  "liftS (read_reg RC_ref) = readS (RC \<circ> regstate)"
+lemma liftS_read_reg_RC[liftState_simp]:
+  "\<lbrakk>read_reg RC_ref\<rbrakk>\<^sub>S = readS (RC \<circ> regstate)"
   by (auto simp: liftState_read_reg_readS register_defs)
 
-lemma liftS_write_reg_RC[simp]:
-  "liftS (write_reg RC_ref v) = updateS (regstate_update (RC_update (\<lambda>_. v)))"
+lemma liftS_write_reg_RC[liftState_simp]:
+  "\<lbrakk>write_reg RC_ref v\<rbrakk>\<^sub>S = updateS (regstate_update (RC_update (\<lambda>_. v)))"
   by (auto simp: liftState_write_reg_updateS register_defs)
 
-lemma liftS_read_reg_RVBAR_EL1[simp]:
-  "liftS (read_reg RVBAR_EL1_ref) = readS (RVBAR_EL1 \<circ> regstate)"
+lemma liftS_read_reg_RVBAR_EL1[liftState_simp]:
+  "\<lbrakk>read_reg RVBAR_EL1_ref\<rbrakk>\<^sub>S = readS (RVBAR_EL1 \<circ> regstate)"
   by (auto simp: liftState_read_reg_readS register_defs)
 
-lemma liftS_write_reg_RVBAR_EL1[simp]:
-  "liftS (write_reg RVBAR_EL1_ref v) = updateS (regstate_update (RVBAR_EL1_update (\<lambda>_. v)))"
+lemma liftS_write_reg_RVBAR_EL1[liftState_simp]:
+  "\<lbrakk>write_reg RVBAR_EL1_ref v\<rbrakk>\<^sub>S = updateS (regstate_update (RVBAR_EL1_update (\<lambda>_. v)))"
   by (auto simp: liftState_write_reg_updateS register_defs)
 
-lemma liftS_read_reg_RVBAR_EL2[simp]:
-  "liftS (read_reg RVBAR_EL2_ref) = readS (RVBAR_EL2 \<circ> regstate)"
+lemma liftS_read_reg_RVBAR_EL2[liftState_simp]:
+  "\<lbrakk>read_reg RVBAR_EL2_ref\<rbrakk>\<^sub>S = readS (RVBAR_EL2 \<circ> regstate)"
   by (auto simp: liftState_read_reg_readS register_defs)
 
-lemma liftS_write_reg_RVBAR_EL2[simp]:
-  "liftS (write_reg RVBAR_EL2_ref v) = updateS (regstate_update (RVBAR_EL2_update (\<lambda>_. v)))"
+lemma liftS_write_reg_RVBAR_EL2[liftState_simp]:
+  "\<lbrakk>write_reg RVBAR_EL2_ref v\<rbrakk>\<^sub>S = updateS (regstate_update (RVBAR_EL2_update (\<lambda>_. v)))"
   by (auto simp: liftState_write_reg_updateS register_defs)
 
-lemma liftS_read_reg_RVBAR_EL3[simp]:
-  "liftS (read_reg RVBAR_EL3_ref) = readS (RVBAR_EL3 \<circ> regstate)"
+lemma liftS_read_reg_RVBAR_EL3[liftState_simp]:
+  "\<lbrakk>read_reg RVBAR_EL3_ref\<rbrakk>\<^sub>S = readS (RVBAR_EL3 \<circ> regstate)"
   by (auto simp: liftState_read_reg_readS register_defs)
 
-lemma liftS_write_reg_RVBAR_EL3[simp]:
-  "liftS (write_reg RVBAR_EL3_ref v) = updateS (regstate_update (RVBAR_EL3_update (\<lambda>_. v)))"
+lemma liftS_write_reg_RVBAR_EL3[liftState_simp]:
+  "\<lbrakk>write_reg RVBAR_EL3_ref v\<rbrakk>\<^sub>S = updateS (regstate_update (RVBAR_EL3_update (\<lambda>_. v)))"
   by (auto simp: liftState_write_reg_updateS register_defs)
 
-lemma liftS_read_reg_SCR[simp]:
-  "liftS (read_reg SCR_ref) = readS (SCR \<circ> regstate)"
+lemma liftS_read_reg_SCR[liftState_simp]:
+  "\<lbrakk>read_reg SCR_ref\<rbrakk>\<^sub>S = readS (SCR \<circ> regstate)"
   by (auto simp: liftState_read_reg_readS register_defs)
 
-lemma liftS_write_reg_SCR[simp]:
-  "liftS (write_reg SCR_ref v) = updateS (regstate_update (SCR_update (\<lambda>_. v)))"
+lemma liftS_write_reg_SCR[liftState_simp]:
+  "\<lbrakk>write_reg SCR_ref v\<rbrakk>\<^sub>S = updateS (regstate_update (SCR_update (\<lambda>_. v)))"
   by (auto simp: liftState_write_reg_updateS register_defs)
 
-lemma liftS_read_reg_SCR_EL3[simp]:
-  "liftS (read_reg SCR_EL3_ref) = readS (SCR_EL3 \<circ> regstate)"
+lemma liftS_read_reg_SCR_EL3[liftState_simp]:
+  "\<lbrakk>read_reg SCR_EL3_ref\<rbrakk>\<^sub>S = readS (SCR_EL3 \<circ> regstate)"
   by (auto simp: liftState_read_reg_readS register_defs)
 
-lemma liftS_write_reg_SCR_EL3[simp]:
-  "liftS (write_reg SCR_EL3_ref v) = updateS (regstate_update (SCR_EL3_update (\<lambda>_. v)))"
+lemma liftS_write_reg_SCR_EL3[liftState_simp]:
+  "\<lbrakk>write_reg SCR_EL3_ref v\<rbrakk>\<^sub>S = updateS (regstate_update (SCR_EL3_update (\<lambda>_. v)))"
   by (auto simp: liftState_write_reg_updateS register_defs)
 
-lemma liftS_read_reg_SCTLR[simp]:
-  "liftS (read_reg SCTLR_ref) = readS (SCTLR \<circ> regstate)"
+lemma liftS_read_reg_SCTLR[liftState_simp]:
+  "\<lbrakk>read_reg SCTLR_ref\<rbrakk>\<^sub>S = readS (SCTLR \<circ> regstate)"
   by (auto simp: liftState_read_reg_readS register_defs)
 
-lemma liftS_write_reg_SCTLR[simp]:
-  "liftS (write_reg SCTLR_ref v) = updateS (regstate_update (SCTLR_update (\<lambda>_. v)))"
+lemma liftS_write_reg_SCTLR[liftState_simp]:
+  "\<lbrakk>write_reg SCTLR_ref v\<rbrakk>\<^sub>S = updateS (regstate_update (SCTLR_update (\<lambda>_. v)))"
   by (auto simp: liftState_write_reg_updateS register_defs)
 
-lemma liftS_read_reg_SCTLR_EL1[simp]:
-  "liftS (read_reg SCTLR_EL1_ref) = readS (SCTLR_EL1 \<circ> regstate)"
+lemma liftS_read_reg_SCTLR_EL1[liftState_simp]:
+  "\<lbrakk>read_reg SCTLR_EL1_ref\<rbrakk>\<^sub>S = readS (SCTLR_EL1 \<circ> regstate)"
   by (auto simp: liftState_read_reg_readS register_defs)
 
-lemma liftS_write_reg_SCTLR_EL1[simp]:
-  "liftS (write_reg SCTLR_EL1_ref v) = updateS (regstate_update (SCTLR_EL1_update (\<lambda>_. v)))"
+lemma liftS_write_reg_SCTLR_EL1[liftState_simp]:
+  "\<lbrakk>write_reg SCTLR_EL1_ref v\<rbrakk>\<^sub>S = updateS (regstate_update (SCTLR_EL1_update (\<lambda>_. v)))"
   by (auto simp: liftState_write_reg_updateS register_defs)
 
-lemma liftS_read_reg_SCTLR_EL2[simp]:
-  "liftS (read_reg SCTLR_EL2_ref) = readS (SCTLR_EL2 \<circ> regstate)"
+lemma liftS_read_reg_SCTLR_EL2[liftState_simp]:
+  "\<lbrakk>read_reg SCTLR_EL2_ref\<rbrakk>\<^sub>S = readS (SCTLR_EL2 \<circ> regstate)"
   by (auto simp: liftState_read_reg_readS register_defs)
 
-lemma liftS_write_reg_SCTLR_EL2[simp]:
-  "liftS (write_reg SCTLR_EL2_ref v) = updateS (regstate_update (SCTLR_EL2_update (\<lambda>_. v)))"
+lemma liftS_write_reg_SCTLR_EL2[liftState_simp]:
+  "\<lbrakk>write_reg SCTLR_EL2_ref v\<rbrakk>\<^sub>S = updateS (regstate_update (SCTLR_EL2_update (\<lambda>_. v)))"
   by (auto simp: liftState_write_reg_updateS register_defs)
 
-lemma liftS_read_reg_SCTLR_EL3[simp]:
-  "liftS (read_reg SCTLR_EL3_ref) = readS (SCTLR_EL3 \<circ> regstate)"
+lemma liftS_read_reg_SCTLR_EL3[liftState_simp]:
+  "\<lbrakk>read_reg SCTLR_EL3_ref\<rbrakk>\<^sub>S = readS (SCTLR_EL3 \<circ> regstate)"
   by (auto simp: liftState_read_reg_readS register_defs)
 
-lemma liftS_write_reg_SCTLR_EL3[simp]:
-  "liftS (write_reg SCTLR_EL3_ref v) = updateS (regstate_update (SCTLR_EL3_update (\<lambda>_. v)))"
+lemma liftS_write_reg_SCTLR_EL3[liftState_simp]:
+  "\<lbrakk>write_reg SCTLR_EL3_ref v\<rbrakk>\<^sub>S = updateS (regstate_update (SCTLR_EL3_update (\<lambda>_. v)))"
   by (auto simp: liftState_write_reg_updateS register_defs)
 
-lemma liftS_read_reg_SDCR[simp]:
-  "liftS (read_reg SDCR_ref) = readS (SDCR \<circ> regstate)"
+lemma liftS_read_reg_SDCR[liftState_simp]:
+  "\<lbrakk>read_reg SDCR_ref\<rbrakk>\<^sub>S = readS (SDCR \<circ> regstate)"
   by (auto simp: liftState_read_reg_readS register_defs)
 
-lemma liftS_write_reg_SDCR[simp]:
-  "liftS (write_reg SDCR_ref v) = updateS (regstate_update (SDCR_update (\<lambda>_. v)))"
+lemma liftS_write_reg_SDCR[liftState_simp]:
+  "\<lbrakk>write_reg SDCR_ref v\<rbrakk>\<^sub>S = updateS (regstate_update (SDCR_update (\<lambda>_. v)))"
   by (auto simp: liftState_write_reg_updateS register_defs)
 
-lemma liftS_read_reg_SDER[simp]:
-  "liftS (read_reg SDER_ref) = readS (SDER \<circ> regstate)"
+lemma liftS_read_reg_SDER[liftState_simp]:
+  "\<lbrakk>read_reg SDER_ref\<rbrakk>\<^sub>S = readS (SDER \<circ> regstate)"
   by (auto simp: liftState_read_reg_readS register_defs)
 
-lemma liftS_write_reg_SDER[simp]:
-  "liftS (write_reg SDER_ref v) = updateS (regstate_update (SDER_update (\<lambda>_. v)))"
+lemma liftS_write_reg_SDER[liftState_simp]:
+  "\<lbrakk>write_reg SDER_ref v\<rbrakk>\<^sub>S = updateS (regstate_update (SDER_update (\<lambda>_. v)))"
   by (auto simp: liftState_write_reg_updateS register_defs)
 
-lemma liftS_read_reg_SPIDEN[simp]:
-  "liftS (read_reg SPIDEN_ref) = readS (SPIDEN \<circ> regstate)"
+lemma liftS_read_reg_SPIDEN[liftState_simp]:
+  "\<lbrakk>read_reg SPIDEN_ref\<rbrakk>\<^sub>S = readS (SPIDEN \<circ> regstate)"
   by (auto simp: liftState_read_reg_readS register_defs)
 
-lemma liftS_write_reg_SPIDEN[simp]:
-  "liftS (write_reg SPIDEN_ref v) = updateS (regstate_update (SPIDEN_update (\<lambda>_. v)))"
+lemma liftS_write_reg_SPIDEN[liftState_simp]:
+  "\<lbrakk>write_reg SPIDEN_ref v\<rbrakk>\<^sub>S = updateS (regstate_update (SPIDEN_update (\<lambda>_. v)))"
   by (auto simp: liftState_write_reg_updateS register_defs)
 
-lemma liftS_read_reg_SPSR_EL1[simp]:
-  "liftS (read_reg SPSR_EL1_ref) = readS (SPSR_EL1 \<circ> regstate)"
+lemma liftS_read_reg_SPSR_EL1[liftState_simp]:
+  "\<lbrakk>read_reg SPSR_EL1_ref\<rbrakk>\<^sub>S = readS (SPSR_EL1 \<circ> regstate)"
   by (auto simp: liftState_read_reg_readS register_defs)
 
-lemma liftS_write_reg_SPSR_EL1[simp]:
-  "liftS (write_reg SPSR_EL1_ref v) = updateS (regstate_update (SPSR_EL1_update (\<lambda>_. v)))"
+lemma liftS_write_reg_SPSR_EL1[liftState_simp]:
+  "\<lbrakk>write_reg SPSR_EL1_ref v\<rbrakk>\<^sub>S = updateS (regstate_update (SPSR_EL1_update (\<lambda>_. v)))"
   by (auto simp: liftState_write_reg_updateS register_defs)
 
-lemma liftS_read_reg_SPSR_EL2[simp]:
-  "liftS (read_reg SPSR_EL2_ref) = readS (SPSR_EL2 \<circ> regstate)"
+lemma liftS_read_reg_SPSR_EL2[liftState_simp]:
+  "\<lbrakk>read_reg SPSR_EL2_ref\<rbrakk>\<^sub>S = readS (SPSR_EL2 \<circ> regstate)"
   by (auto simp: liftState_read_reg_readS register_defs)
 
-lemma liftS_write_reg_SPSR_EL2[simp]:
-  "liftS (write_reg SPSR_EL2_ref v) = updateS (regstate_update (SPSR_EL2_update (\<lambda>_. v)))"
+lemma liftS_write_reg_SPSR_EL2[liftState_simp]:
+  "\<lbrakk>write_reg SPSR_EL2_ref v\<rbrakk>\<^sub>S = updateS (regstate_update (SPSR_EL2_update (\<lambda>_. v)))"
   by (auto simp: liftState_write_reg_updateS register_defs)
 
-lemma liftS_read_reg_SPSR_EL3[simp]:
-  "liftS (read_reg SPSR_EL3_ref) = readS (SPSR_EL3 \<circ> regstate)"
+lemma liftS_read_reg_SPSR_EL3[liftState_simp]:
+  "\<lbrakk>read_reg SPSR_EL3_ref\<rbrakk>\<^sub>S = readS (SPSR_EL3 \<circ> regstate)"
   by (auto simp: liftState_read_reg_readS register_defs)
 
-lemma liftS_write_reg_SPSR_EL3[simp]:
-  "liftS (write_reg SPSR_EL3_ref v) = updateS (regstate_update (SPSR_EL3_update (\<lambda>_. v)))"
+lemma liftS_write_reg_SPSR_EL3[liftState_simp]:
+  "\<lbrakk>write_reg SPSR_EL3_ref v\<rbrakk>\<^sub>S = updateS (regstate_update (SPSR_EL3_update (\<lambda>_. v)))"
   by (auto simp: liftState_write_reg_updateS register_defs)
 
-lemma liftS_read_reg_SPSR_abt[simp]:
-  "liftS (read_reg SPSR_abt_ref) = readS (SPSR_abt \<circ> regstate)"
+lemma liftS_read_reg_SPSR_abt[liftState_simp]:
+  "\<lbrakk>read_reg SPSR_abt_ref\<rbrakk>\<^sub>S = readS (SPSR_abt \<circ> regstate)"
   by (auto simp: liftState_read_reg_readS register_defs)
 
-lemma liftS_write_reg_SPSR_abt[simp]:
-  "liftS (write_reg SPSR_abt_ref v) = updateS (regstate_update (SPSR_abt_update (\<lambda>_. v)))"
+lemma liftS_write_reg_SPSR_abt[liftState_simp]:
+  "\<lbrakk>write_reg SPSR_abt_ref v\<rbrakk>\<^sub>S = updateS (regstate_update (SPSR_abt_update (\<lambda>_. v)))"
   by (auto simp: liftState_write_reg_updateS register_defs)
 
-lemma liftS_read_reg_SPSR_fiq[simp]:
-  "liftS (read_reg SPSR_fiq_ref) = readS (SPSR_fiq \<circ> regstate)"
+lemma liftS_read_reg_SPSR_fiq[liftState_simp]:
+  "\<lbrakk>read_reg SPSR_fiq_ref\<rbrakk>\<^sub>S = readS (SPSR_fiq \<circ> regstate)"
   by (auto simp: liftState_read_reg_readS register_defs)
 
-lemma liftS_write_reg_SPSR_fiq[simp]:
-  "liftS (write_reg SPSR_fiq_ref v) = updateS (regstate_update (SPSR_fiq_update (\<lambda>_. v)))"
+lemma liftS_write_reg_SPSR_fiq[liftState_simp]:
+  "\<lbrakk>write_reg SPSR_fiq_ref v\<rbrakk>\<^sub>S = updateS (regstate_update (SPSR_fiq_update (\<lambda>_. v)))"
   by (auto simp: liftState_write_reg_updateS register_defs)
 
-lemma liftS_read_reg_SPSR_hyp[simp]:
-  "liftS (read_reg SPSR_hyp_ref) = readS (SPSR_hyp \<circ> regstate)"
+lemma liftS_read_reg_SPSR_hyp[liftState_simp]:
+  "\<lbrakk>read_reg SPSR_hyp_ref\<rbrakk>\<^sub>S = readS (SPSR_hyp \<circ> regstate)"
   by (auto simp: liftState_read_reg_readS register_defs)
 
-lemma liftS_write_reg_SPSR_hyp[simp]:
-  "liftS (write_reg SPSR_hyp_ref v) = updateS (regstate_update (SPSR_hyp_update (\<lambda>_. v)))"
+lemma liftS_write_reg_SPSR_hyp[liftState_simp]:
+  "\<lbrakk>write_reg SPSR_hyp_ref v\<rbrakk>\<^sub>S = updateS (regstate_update (SPSR_hyp_update (\<lambda>_. v)))"
   by (auto simp: liftState_write_reg_updateS register_defs)
 
-lemma liftS_read_reg_SPSR_irq[simp]:
-  "liftS (read_reg SPSR_irq_ref) = readS (SPSR_irq \<circ> regstate)"
+lemma liftS_read_reg_SPSR_irq[liftState_simp]:
+  "\<lbrakk>read_reg SPSR_irq_ref\<rbrakk>\<^sub>S = readS (SPSR_irq \<circ> regstate)"
   by (auto simp: liftState_read_reg_readS register_defs)
 
-lemma liftS_write_reg_SPSR_irq[simp]:
-  "liftS (write_reg SPSR_irq_ref v) = updateS (regstate_update (SPSR_irq_update (\<lambda>_. v)))"
+lemma liftS_write_reg_SPSR_irq[liftState_simp]:
+  "\<lbrakk>write_reg SPSR_irq_ref v\<rbrakk>\<^sub>S = updateS (regstate_update (SPSR_irq_update (\<lambda>_. v)))"
   by (auto simp: liftState_write_reg_updateS register_defs)
 
-lemma liftS_read_reg_SPSR_mon[simp]:
-  "liftS (read_reg SPSR_mon_ref) = readS (SPSR_mon \<circ> regstate)"
+lemma liftS_read_reg_SPSR_mon[liftState_simp]:
+  "\<lbrakk>read_reg SPSR_mon_ref\<rbrakk>\<^sub>S = readS (SPSR_mon \<circ> regstate)"
   by (auto simp: liftState_read_reg_readS register_defs)
 
-lemma liftS_write_reg_SPSR_mon[simp]:
-  "liftS (write_reg SPSR_mon_ref v) = updateS (regstate_update (SPSR_mon_update (\<lambda>_. v)))"
+lemma liftS_write_reg_SPSR_mon[liftState_simp]:
+  "\<lbrakk>write_reg SPSR_mon_ref v\<rbrakk>\<^sub>S = updateS (regstate_update (SPSR_mon_update (\<lambda>_. v)))"
   by (auto simp: liftState_write_reg_updateS register_defs)
 
-lemma liftS_read_reg_SPSR_svc[simp]:
-  "liftS (read_reg SPSR_svc_ref) = readS (SPSR_svc \<circ> regstate)"
+lemma liftS_read_reg_SPSR_svc[liftState_simp]:
+  "\<lbrakk>read_reg SPSR_svc_ref\<rbrakk>\<^sub>S = readS (SPSR_svc \<circ> regstate)"
   by (auto simp: liftState_read_reg_readS register_defs)
 
-lemma liftS_write_reg_SPSR_svc[simp]:
-  "liftS (write_reg SPSR_svc_ref v) = updateS (regstate_update (SPSR_svc_update (\<lambda>_. v)))"
+lemma liftS_write_reg_SPSR_svc[liftState_simp]:
+  "\<lbrakk>write_reg SPSR_svc_ref v\<rbrakk>\<^sub>S = updateS (regstate_update (SPSR_svc_update (\<lambda>_. v)))"
   by (auto simp: liftState_write_reg_updateS register_defs)
 
-lemma liftS_read_reg_SPSR_und[simp]:
-  "liftS (read_reg SPSR_und_ref) = readS (SPSR_und \<circ> regstate)"
+lemma liftS_read_reg_SPSR_und[liftState_simp]:
+  "\<lbrakk>read_reg SPSR_und_ref\<rbrakk>\<^sub>S = readS (SPSR_und \<circ> regstate)"
   by (auto simp: liftState_read_reg_readS register_defs)
 
-lemma liftS_write_reg_SPSR_und[simp]:
-  "liftS (write_reg SPSR_und_ref v) = updateS (regstate_update (SPSR_und_update (\<lambda>_. v)))"
+lemma liftS_write_reg_SPSR_und[liftState_simp]:
+  "\<lbrakk>write_reg SPSR_und_ref v\<rbrakk>\<^sub>S = updateS (regstate_update (SPSR_und_update (\<lambda>_. v)))"
   by (auto simp: liftState_write_reg_updateS register_defs)
 
-lemma liftS_read_reg_SP_EL0[simp]:
-  "liftS (read_reg SP_EL0_ref) = readS (SP_EL0 \<circ> regstate)"
+lemma liftS_read_reg_SP_EL0[liftState_simp]:
+  "\<lbrakk>read_reg SP_EL0_ref\<rbrakk>\<^sub>S = readS (SP_EL0 \<circ> regstate)"
   by (auto simp: liftState_read_reg_readS register_defs)
 
-lemma liftS_write_reg_SP_EL0[simp]:
-  "liftS (write_reg SP_EL0_ref v) = updateS (regstate_update (SP_EL0_update (\<lambda>_. v)))"
+lemma liftS_write_reg_SP_EL0[liftState_simp]:
+  "\<lbrakk>write_reg SP_EL0_ref v\<rbrakk>\<^sub>S = updateS (regstate_update (SP_EL0_update (\<lambda>_. v)))"
   by (auto simp: liftState_write_reg_updateS register_defs)
 
-lemma liftS_read_reg_SP_EL1[simp]:
-  "liftS (read_reg SP_EL1_ref) = readS (SP_EL1 \<circ> regstate)"
+lemma liftS_read_reg_SP_EL1[liftState_simp]:
+  "\<lbrakk>read_reg SP_EL1_ref\<rbrakk>\<^sub>S = readS (SP_EL1 \<circ> regstate)"
   by (auto simp: liftState_read_reg_readS register_defs)
 
-lemma liftS_write_reg_SP_EL1[simp]:
-  "liftS (write_reg SP_EL1_ref v) = updateS (regstate_update (SP_EL1_update (\<lambda>_. v)))"
+lemma liftS_write_reg_SP_EL1[liftState_simp]:
+  "\<lbrakk>write_reg SP_EL1_ref v\<rbrakk>\<^sub>S = updateS (regstate_update (SP_EL1_update (\<lambda>_. v)))"
   by (auto simp: liftState_write_reg_updateS register_defs)
 
-lemma liftS_read_reg_SP_EL2[simp]:
-  "liftS (read_reg SP_EL2_ref) = readS (SP_EL2 \<circ> regstate)"
+lemma liftS_read_reg_SP_EL2[liftState_simp]:
+  "\<lbrakk>read_reg SP_EL2_ref\<rbrakk>\<^sub>S = readS (SP_EL2 \<circ> regstate)"
   by (auto simp: liftState_read_reg_readS register_defs)
 
-lemma liftS_write_reg_SP_EL2[simp]:
-  "liftS (write_reg SP_EL2_ref v) = updateS (regstate_update (SP_EL2_update (\<lambda>_. v)))"
+lemma liftS_write_reg_SP_EL2[liftState_simp]:
+  "\<lbrakk>write_reg SP_EL2_ref v\<rbrakk>\<^sub>S = updateS (regstate_update (SP_EL2_update (\<lambda>_. v)))"
   by (auto simp: liftState_write_reg_updateS register_defs)
 
-lemma liftS_read_reg_SP_EL3[simp]:
-  "liftS (read_reg SP_EL3_ref) = readS (SP_EL3 \<circ> regstate)"
+lemma liftS_read_reg_SP_EL3[liftState_simp]:
+  "\<lbrakk>read_reg SP_EL3_ref\<rbrakk>\<^sub>S = readS (SP_EL3 \<circ> regstate)"
   by (auto simp: liftState_read_reg_readS register_defs)
 
-lemma liftS_write_reg_SP_EL3[simp]:
-  "liftS (write_reg SP_EL3_ref v) = updateS (regstate_update (SP_EL3_update (\<lambda>_. v)))"
+lemma liftS_write_reg_SP_EL3[liftState_simp]:
+  "\<lbrakk>write_reg SP_EL3_ref v\<rbrakk>\<^sub>S = updateS (regstate_update (SP_EL3_update (\<lambda>_. v)))"
   by (auto simp: liftState_write_reg_updateS register_defs)
 
-lemma liftS_read_reg_SP_mon[simp]:
-  "liftS (read_reg SP_mon_ref) = readS (SP_mon \<circ> regstate)"
+lemma liftS_read_reg_SP_mon[liftState_simp]:
+  "\<lbrakk>read_reg SP_mon_ref\<rbrakk>\<^sub>S = readS (SP_mon \<circ> regstate)"
   by (auto simp: liftState_read_reg_readS register_defs)
 
-lemma liftS_write_reg_SP_mon[simp]:
-  "liftS (write_reg SP_mon_ref v) = updateS (regstate_update (SP_mon_update (\<lambda>_. v)))"
+lemma liftS_write_reg_SP_mon[liftState_simp]:
+  "\<lbrakk>write_reg SP_mon_ref v\<rbrakk>\<^sub>S = updateS (regstate_update (SP_mon_update (\<lambda>_. v)))"
   by (auto simp: liftState_write_reg_updateS register_defs)
 
-lemma liftS_read_reg_TCR_EL1[simp]:
-  "liftS (read_reg TCR_EL1_ref) = readS (TCR_EL1 \<circ> regstate)"
+lemma liftS_read_reg_TCR_EL1[liftState_simp]:
+  "\<lbrakk>read_reg TCR_EL1_ref\<rbrakk>\<^sub>S = readS (TCR_EL1 \<circ> regstate)"
   by (auto simp: liftState_read_reg_readS register_defs)
 
-lemma liftS_write_reg_TCR_EL1[simp]:
-  "liftS (write_reg TCR_EL1_ref v) = updateS (regstate_update (TCR_EL1_update (\<lambda>_. v)))"
+lemma liftS_write_reg_TCR_EL1[liftState_simp]:
+  "\<lbrakk>write_reg TCR_EL1_ref v\<rbrakk>\<^sub>S = updateS (regstate_update (TCR_EL1_update (\<lambda>_. v)))"
   by (auto simp: liftState_write_reg_updateS register_defs)
 
-lemma liftS_read_reg_TCR_EL2[simp]:
-  "liftS (read_reg TCR_EL2_ref) = readS (TCR_EL2 \<circ> regstate)"
+lemma liftS_read_reg_TCR_EL2[liftState_simp]:
+  "\<lbrakk>read_reg TCR_EL2_ref\<rbrakk>\<^sub>S = readS (TCR_EL2 \<circ> regstate)"
   by (auto simp: liftState_read_reg_readS register_defs)
 
-lemma liftS_write_reg_TCR_EL2[simp]:
-  "liftS (write_reg TCR_EL2_ref v) = updateS (regstate_update (TCR_EL2_update (\<lambda>_. v)))"
+lemma liftS_write_reg_TCR_EL2[liftState_simp]:
+  "\<lbrakk>write_reg TCR_EL2_ref v\<rbrakk>\<^sub>S = updateS (regstate_update (TCR_EL2_update (\<lambda>_. v)))"
   by (auto simp: liftState_write_reg_updateS register_defs)
 
-lemma liftS_read_reg_TCR_EL3[simp]:
-  "liftS (read_reg TCR_EL3_ref) = readS (TCR_EL3 \<circ> regstate)"
+lemma liftS_read_reg_TCR_EL3[liftState_simp]:
+  "\<lbrakk>read_reg TCR_EL3_ref\<rbrakk>\<^sub>S = readS (TCR_EL3 \<circ> regstate)"
   by (auto simp: liftState_read_reg_readS register_defs)
 
-lemma liftS_write_reg_TCR_EL3[simp]:
-  "liftS (write_reg TCR_EL3_ref v) = updateS (regstate_update (TCR_EL3_update (\<lambda>_. v)))"
+lemma liftS_write_reg_TCR_EL3[liftState_simp]:
+  "\<lbrakk>write_reg TCR_EL3_ref v\<rbrakk>\<^sub>S = updateS (regstate_update (TCR_EL3_update (\<lambda>_. v)))"
   by (auto simp: liftState_write_reg_updateS register_defs)
 
-lemma liftS_read_reg_TTBCR[simp]:
-  "liftS (read_reg TTBCR_ref) = readS (TTBCR \<circ> regstate)"
+lemma liftS_read_reg_TTBCR[liftState_simp]:
+  "\<lbrakk>read_reg TTBCR_ref\<rbrakk>\<^sub>S = readS (TTBCR \<circ> regstate)"
   by (auto simp: liftState_read_reg_readS register_defs)
 
-lemma liftS_write_reg_TTBCR[simp]:
-  "liftS (write_reg TTBCR_ref v) = updateS (regstate_update (TTBCR_update (\<lambda>_. v)))"
+lemma liftS_write_reg_TTBCR[liftState_simp]:
+  "\<lbrakk>write_reg TTBCR_ref v\<rbrakk>\<^sub>S = updateS (regstate_update (TTBCR_update (\<lambda>_. v)))"
   by (auto simp: liftState_write_reg_updateS register_defs)
 
-lemma liftS_read_reg_TTBR0_EL1[simp]:
-  "liftS (read_reg TTBR0_EL1_ref) = readS (TTBR0_EL1 \<circ> regstate)"
+lemma liftS_read_reg_TTBR0_EL1[liftState_simp]:
+  "\<lbrakk>read_reg TTBR0_EL1_ref\<rbrakk>\<^sub>S = readS (TTBR0_EL1 \<circ> regstate)"
   by (auto simp: liftState_read_reg_readS register_defs)
 
-lemma liftS_write_reg_TTBR0_EL1[simp]:
-  "liftS (write_reg TTBR0_EL1_ref v) = updateS (regstate_update (TTBR0_EL1_update (\<lambda>_. v)))"
+lemma liftS_write_reg_TTBR0_EL1[liftState_simp]:
+  "\<lbrakk>write_reg TTBR0_EL1_ref v\<rbrakk>\<^sub>S = updateS (regstate_update (TTBR0_EL1_update (\<lambda>_. v)))"
   by (auto simp: liftState_write_reg_updateS register_defs)
 
-lemma liftS_read_reg_TTBR0_EL2[simp]:
-  "liftS (read_reg TTBR0_EL2_ref) = readS (TTBR0_EL2 \<circ> regstate)"
+lemma liftS_read_reg_TTBR0_EL2[liftState_simp]:
+  "\<lbrakk>read_reg TTBR0_EL2_ref\<rbrakk>\<^sub>S = readS (TTBR0_EL2 \<circ> regstate)"
   by (auto simp: liftState_read_reg_readS register_defs)
 
-lemma liftS_write_reg_TTBR0_EL2[simp]:
-  "liftS (write_reg TTBR0_EL2_ref v) = updateS (regstate_update (TTBR0_EL2_update (\<lambda>_. v)))"
+lemma liftS_write_reg_TTBR0_EL2[liftState_simp]:
+  "\<lbrakk>write_reg TTBR0_EL2_ref v\<rbrakk>\<^sub>S = updateS (regstate_update (TTBR0_EL2_update (\<lambda>_. v)))"
   by (auto simp: liftState_write_reg_updateS register_defs)
 
-lemma liftS_read_reg_TTBR0_EL3[simp]:
-  "liftS (read_reg TTBR0_EL3_ref) = readS (TTBR0_EL3 \<circ> regstate)"
+lemma liftS_read_reg_TTBR0_EL3[liftState_simp]:
+  "\<lbrakk>read_reg TTBR0_EL3_ref\<rbrakk>\<^sub>S = readS (TTBR0_EL3 \<circ> regstate)"
   by (auto simp: liftState_read_reg_readS register_defs)
 
-lemma liftS_write_reg_TTBR0_EL3[simp]:
-  "liftS (write_reg TTBR0_EL3_ref v) = updateS (regstate_update (TTBR0_EL3_update (\<lambda>_. v)))"
+lemma liftS_write_reg_TTBR0_EL3[liftState_simp]:
+  "\<lbrakk>write_reg TTBR0_EL3_ref v\<rbrakk>\<^sub>S = updateS (regstate_update (TTBR0_EL3_update (\<lambda>_. v)))"
   by (auto simp: liftState_write_reg_updateS register_defs)
 
-lemma liftS_read_reg_TTBR1_EL1[simp]:
-  "liftS (read_reg TTBR1_EL1_ref) = readS (TTBR1_EL1 \<circ> regstate)"
+lemma liftS_read_reg_TTBR1_EL1[liftState_simp]:
+  "\<lbrakk>read_reg TTBR1_EL1_ref\<rbrakk>\<^sub>S = readS (TTBR1_EL1 \<circ> regstate)"
   by (auto simp: liftState_read_reg_readS register_defs)
 
-lemma liftS_write_reg_TTBR1_EL1[simp]:
-  "liftS (write_reg TTBR1_EL1_ref v) = updateS (regstate_update (TTBR1_EL1_update (\<lambda>_. v)))"
+lemma liftS_write_reg_TTBR1_EL1[liftState_simp]:
+  "\<lbrakk>write_reg TTBR1_EL1_ref v\<rbrakk>\<^sub>S = updateS (regstate_update (TTBR1_EL1_update (\<lambda>_. v)))"
   by (auto simp: liftState_write_reg_updateS register_defs)
 
-lemma liftS_read_reg_TTBR1_EL2[simp]:
-  "liftS (read_reg TTBR1_EL2_ref) = readS (TTBR1_EL2 \<circ> regstate)"
+lemma liftS_read_reg_TTBR1_EL2[liftState_simp]:
+  "\<lbrakk>read_reg TTBR1_EL2_ref\<rbrakk>\<^sub>S = readS (TTBR1_EL2 \<circ> regstate)"
   by (auto simp: liftState_read_reg_readS register_defs)
 
-lemma liftS_write_reg_TTBR1_EL2[simp]:
-  "liftS (write_reg TTBR1_EL2_ref v) = updateS (regstate_update (TTBR1_EL2_update (\<lambda>_. v)))"
+lemma liftS_write_reg_TTBR1_EL2[liftState_simp]:
+  "\<lbrakk>write_reg TTBR1_EL2_ref v\<rbrakk>\<^sub>S = updateS (regstate_update (TTBR1_EL2_update (\<lambda>_. v)))"
   by (auto simp: liftState_write_reg_updateS register_defs)
 
-lemma liftS_read_reg_VBAR[simp]:
-  "liftS (read_reg VBAR_ref) = readS (VBAR \<circ> regstate)"
+lemma liftS_read_reg_VBAR[liftState_simp]:
+  "\<lbrakk>read_reg VBAR_ref\<rbrakk>\<^sub>S = readS (VBAR \<circ> regstate)"
   by (auto simp: liftState_read_reg_readS register_defs)
 
-lemma liftS_write_reg_VBAR[simp]:
-  "liftS (write_reg VBAR_ref v) = updateS (regstate_update (VBAR_update (\<lambda>_. v)))"
+lemma liftS_write_reg_VBAR[liftState_simp]:
+  "\<lbrakk>write_reg VBAR_ref v\<rbrakk>\<^sub>S = updateS (regstate_update (VBAR_update (\<lambda>_. v)))"
   by (auto simp: liftState_write_reg_updateS register_defs)
 
-lemma liftS_read_reg_VBAR_EL1[simp]:
-  "liftS (read_reg VBAR_EL1_ref) = readS (VBAR_EL1 \<circ> regstate)"
+lemma liftS_read_reg_VBAR_EL1[liftState_simp]:
+  "\<lbrakk>read_reg VBAR_EL1_ref\<rbrakk>\<^sub>S = readS (VBAR_EL1 \<circ> regstate)"
   by (auto simp: liftState_read_reg_readS register_defs)
 
-lemma liftS_write_reg_VBAR_EL1[simp]:
-  "liftS (write_reg VBAR_EL1_ref v) = updateS (regstate_update (VBAR_EL1_update (\<lambda>_. v)))"
+lemma liftS_write_reg_VBAR_EL1[liftState_simp]:
+  "\<lbrakk>write_reg VBAR_EL1_ref v\<rbrakk>\<^sub>S = updateS (regstate_update (VBAR_EL1_update (\<lambda>_. v)))"
   by (auto simp: liftState_write_reg_updateS register_defs)
 
-lemma liftS_read_reg_VBAR_EL2[simp]:
-  "liftS (read_reg VBAR_EL2_ref) = readS (VBAR_EL2 \<circ> regstate)"
+lemma liftS_read_reg_VBAR_EL2[liftState_simp]:
+  "\<lbrakk>read_reg VBAR_EL2_ref\<rbrakk>\<^sub>S = readS (VBAR_EL2 \<circ> regstate)"
   by (auto simp: liftState_read_reg_readS register_defs)
 
-lemma liftS_write_reg_VBAR_EL2[simp]:
-  "liftS (write_reg VBAR_EL2_ref v) = updateS (regstate_update (VBAR_EL2_update (\<lambda>_. v)))"
+lemma liftS_write_reg_VBAR_EL2[liftState_simp]:
+  "\<lbrakk>write_reg VBAR_EL2_ref v\<rbrakk>\<^sub>S = updateS (regstate_update (VBAR_EL2_update (\<lambda>_. v)))"
   by (auto simp: liftState_write_reg_updateS register_defs)
 
-lemma liftS_read_reg_VBAR_EL3[simp]:
-  "liftS (read_reg VBAR_EL3_ref) = readS (VBAR_EL3 \<circ> regstate)"
+lemma liftS_read_reg_VBAR_EL3[liftState_simp]:
+  "\<lbrakk>read_reg VBAR_EL3_ref\<rbrakk>\<^sub>S = readS (VBAR_EL3 \<circ> regstate)"
   by (auto simp: liftState_read_reg_readS register_defs)
 
-lemma liftS_write_reg_VBAR_EL3[simp]:
-  "liftS (write_reg VBAR_EL3_ref v) = updateS (regstate_update (VBAR_EL3_update (\<lambda>_. v)))"
+lemma liftS_write_reg_VBAR_EL3[liftState_simp]:
+  "\<lbrakk>write_reg VBAR_EL3_ref v\<rbrakk>\<^sub>S = updateS (regstate_update (VBAR_EL3_update (\<lambda>_. v)))"
   by (auto simp: liftState_write_reg_updateS register_defs)
 
-lemma liftS_read_reg_VDFSR[simp]:
-  "liftS (read_reg VDFSR_ref) = readS (VDFSR \<circ> regstate)"
+lemma liftS_read_reg_VDFSR[liftState_simp]:
+  "\<lbrakk>read_reg VDFSR_ref\<rbrakk>\<^sub>S = readS (VDFSR \<circ> regstate)"
   by (auto simp: liftState_read_reg_readS register_defs)
 
-lemma liftS_write_reg_VDFSR[simp]:
-  "liftS (write_reg VDFSR_ref v) = updateS (regstate_update (VDFSR_update (\<lambda>_. v)))"
+lemma liftS_write_reg_VDFSR[liftState_simp]:
+  "\<lbrakk>write_reg VDFSR_ref v\<rbrakk>\<^sub>S = updateS (regstate_update (VDFSR_update (\<lambda>_. v)))"
   by (auto simp: liftState_write_reg_updateS register_defs)
 
-lemma liftS_read_reg_VSESR_EL2[simp]:
-  "liftS (read_reg VSESR_EL2_ref) = readS (VSESR_EL2 \<circ> regstate)"
+lemma liftS_read_reg_VSESR_EL2[liftState_simp]:
+  "\<lbrakk>read_reg VSESR_EL2_ref\<rbrakk>\<^sub>S = readS (VSESR_EL2 \<circ> regstate)"
   by (auto simp: liftState_read_reg_readS register_defs)
 
-lemma liftS_write_reg_VSESR_EL2[simp]:
-  "liftS (write_reg VSESR_EL2_ref v) = updateS (regstate_update (VSESR_EL2_update (\<lambda>_. v)))"
+lemma liftS_write_reg_VSESR_EL2[liftState_simp]:
+  "\<lbrakk>write_reg VSESR_EL2_ref v\<rbrakk>\<^sub>S = updateS (regstate_update (VSESR_EL2_update (\<lambda>_. v)))"
   by (auto simp: liftState_write_reg_updateS register_defs)
 
-lemma liftS_read_reg_VTCR_EL2[simp]:
-  "liftS (read_reg VTCR_EL2_ref) = readS (VTCR_EL2 \<circ> regstate)"
+lemma liftS_read_reg_VTCR_EL2[liftState_simp]:
+  "\<lbrakk>read_reg VTCR_EL2_ref\<rbrakk>\<^sub>S = readS (VTCR_EL2 \<circ> regstate)"
   by (auto simp: liftState_read_reg_readS register_defs)
 
-lemma liftS_write_reg_VTCR_EL2[simp]:
-  "liftS (write_reg VTCR_EL2_ref v) = updateS (regstate_update (VTCR_EL2_update (\<lambda>_. v)))"
+lemma liftS_write_reg_VTCR_EL2[liftState_simp]:
+  "\<lbrakk>write_reg VTCR_EL2_ref v\<rbrakk>\<^sub>S = updateS (regstate_update (VTCR_EL2_update (\<lambda>_. v)))"
   by (auto simp: liftState_write_reg_updateS register_defs)
 
-lemma liftS_read_reg_VTTBR_EL2[simp]:
-  "liftS (read_reg VTTBR_EL2_ref) = readS (VTTBR_EL2 \<circ> regstate)"
+lemma liftS_read_reg_VTTBR_EL2[liftState_simp]:
+  "\<lbrakk>read_reg VTTBR_EL2_ref\<rbrakk>\<^sub>S = readS (VTTBR_EL2 \<circ> regstate)"
   by (auto simp: liftState_read_reg_readS register_defs)
 
-lemma liftS_write_reg_VTTBR_EL2[simp]:
-  "liftS (write_reg VTTBR_EL2_ref v) = updateS (regstate_update (VTTBR_EL2_update (\<lambda>_. v)))"
+lemma liftS_write_reg_VTTBR_EL2[liftState_simp]:
+  "\<lbrakk>write_reg VTTBR_EL2_ref v\<rbrakk>\<^sub>S = updateS (regstate_update (VTTBR_EL2_update (\<lambda>_. v)))"
   by (auto simp: liftState_write_reg_updateS register_defs)
 
-lemma liftS_read_reg_PC[simp]:
-  "liftS (read_reg PC_ref) = readS (PC \<circ> regstate)"
+lemma liftS_read_reg_PC[liftState_simp]:
+  "\<lbrakk>read_reg PC_ref\<rbrakk>\<^sub>S = readS (PC \<circ> regstate)"
   by (auto simp: liftState_read_reg_readS register_defs)
 
-lemma liftS_write_reg_PC[simp]:
-  "liftS (write_reg PC_ref v) = updateS (regstate_update (PC_update (\<lambda>_. v)))"
+lemma liftS_write_reg_PC[liftState_simp]:
+  "\<lbrakk>write_reg PC_ref v\<rbrakk>\<^sub>S = updateS (regstate_update (PC_update (\<lambda>_. v)))"
   by (auto simp: liftState_write_reg_updateS register_defs)
 
-lemma liftS_read_reg_R[simp]:
-  "liftS (read_reg R_ref) = readS (R \<circ> regstate)"
+lemma liftS_read_reg_R[liftState_simp]:
+  "\<lbrakk>read_reg R_ref\<rbrakk>\<^sub>S = readS (R \<circ> regstate)"
   by (auto simp: liftState_read_reg_readS register_defs)
 
-lemma liftS_write_reg_R[simp]:
-  "liftS (write_reg R_ref v) = updateS (regstate_update (R_update (\<lambda>_. v)))"
+lemma liftS_write_reg_R[liftState_simp]:
+  "\<lbrakk>write_reg R_ref v\<rbrakk>\<^sub>S = updateS (regstate_update (R_update (\<lambda>_. v)))"
   by (auto simp: liftState_write_reg_updateS register_defs)
 
-lemma liftS_read_reg_V[simp]:
-  "liftS (read_reg V_ref) = readS (V \<circ> regstate)"
+lemma liftS_read_reg_V[liftState_simp]:
+  "\<lbrakk>read_reg V_ref\<rbrakk>\<^sub>S = readS (V \<circ> regstate)"
   by (auto simp: liftState_read_reg_readS register_defs)
 
-lemma liftS_write_reg_V[simp]:
-  "liftS (write_reg V_ref v) = updateS (regstate_update (V_update (\<lambda>_. v)))"
+lemma liftS_write_reg_V[liftState_simp]:
+  "\<lbrakk>write_reg V_ref v\<rbrakk>\<^sub>S = updateS (regstate_update (V_update (\<lambda>_. v)))"
   by (auto simp: liftState_write_reg_updateS register_defs)
 
-lemma liftS_read_reg_BranchTaken[simp]:
-  "liftS (read_reg BranchTaken_ref) = readS (BranchTaken \<circ> regstate)"
+lemma liftS_read_reg_BranchTaken[liftState_simp]:
+  "\<lbrakk>read_reg BranchTaken_ref\<rbrakk>\<^sub>S = readS (BranchTaken \<circ> regstate)"
   by (auto simp: liftState_read_reg_readS register_defs)
 
-lemma liftS_write_reg_BranchTaken[simp]:
-  "liftS (write_reg BranchTaken_ref v) = updateS (regstate_update (BranchTaken_update (\<lambda>_. v)))"
+lemma liftS_write_reg_BranchTaken[liftState_simp]:
+  "\<lbrakk>write_reg BranchTaken_ref v\<rbrakk>\<^sub>S = updateS (regstate_update (BranchTaken_update (\<lambda>_. v)))"
   by (auto simp: liftState_write_reg_updateS register_defs)
 
-lemma liftS_read_reg_ExclusiveLocal[simp]:
-  "liftS (read_reg ExclusiveLocal_ref) = readS (ExclusiveLocal \<circ> regstate)"
+lemma liftS_read_reg_ExclusiveLocal[liftState_simp]:
+  "\<lbrakk>read_reg ExclusiveLocal_ref\<rbrakk>\<^sub>S = readS (ExclusiveLocal \<circ> regstate)"
   by (auto simp: liftState_read_reg_readS register_defs)
 
-lemma liftS_write_reg_ExclusiveLocal[simp]:
-  "liftS (write_reg ExclusiveLocal_ref v) = updateS (regstate_update (ExclusiveLocal_update (\<lambda>_. v)))"
+lemma liftS_write_reg_ExclusiveLocal[liftState_simp]:
+  "\<lbrakk>write_reg ExclusiveLocal_ref v\<rbrakk>\<^sub>S = updateS (regstate_update (ExclusiveLocal_update (\<lambda>_. v)))"
   by (auto simp: liftState_write_reg_updateS register_defs)
 
-lemma liftS_read_reg_Memory[simp]:
-  "liftS (read_reg Memory_ref) = readS (Memory \<circ> regstate)"
+lemma liftS_read_reg_Memory[liftState_simp]:
+  "\<lbrakk>read_reg Memory_ref\<rbrakk>\<^sub>S = readS (Memory \<circ> regstate)"
   by (auto simp: liftState_read_reg_readS register_defs)
 
-lemma liftS_write_reg_Memory[simp]:
-  "liftS (write_reg Memory_ref v) = updateS (regstate_update (Memory_update (\<lambda>_. v)))"
+lemma liftS_write_reg_Memory[liftState_simp]:
+  "\<lbrakk>write_reg Memory_ref v\<rbrakk>\<^sub>S = updateS (regstate_update (Memory_update (\<lambda>_. v)))"
   by (auto simp: liftState_write_reg_updateS register_defs)
 
-lemma liftS_read_reg_PendingInterrupt[simp]:
-  "liftS (read_reg PendingInterrupt_ref) = readS (PendingInterrupt \<circ> regstate)"
+lemma liftS_read_reg_PendingInterrupt[liftState_simp]:
+  "\<lbrakk>read_reg PendingInterrupt_ref\<rbrakk>\<^sub>S = readS (PendingInterrupt \<circ> regstate)"
   by (auto simp: liftState_read_reg_readS register_defs)
 
-lemma liftS_write_reg_PendingInterrupt[simp]:
-  "liftS (write_reg PendingInterrupt_ref v) = updateS (regstate_update (PendingInterrupt_update (\<lambda>_. v)))"
+lemma liftS_write_reg_PendingInterrupt[liftState_simp]:
+  "\<lbrakk>write_reg PendingInterrupt_ref v\<rbrakk>\<^sub>S = updateS (regstate_update (PendingInterrupt_update (\<lambda>_. v)))"
   by (auto simp: liftState_write_reg_updateS register_defs)
 
-lemma liftS_read_reg_PendingPhysicalSError[simp]:
-  "liftS (read_reg PendingPhysicalSError_ref) = readS (PendingPhysicalSError \<circ> regstate)"
+lemma liftS_read_reg_PendingPhysicalSError[liftState_simp]:
+  "\<lbrakk>read_reg PendingPhysicalSError_ref\<rbrakk>\<^sub>S = readS (PendingPhysicalSError \<circ> regstate)"
   by (auto simp: liftState_read_reg_readS register_defs)
 
-lemma liftS_write_reg_PendingPhysicalSError[simp]:
-  "liftS (write_reg PendingPhysicalSError_ref v) = updateS (regstate_update (PendingPhysicalSError_update (\<lambda>_. v)))"
+lemma liftS_write_reg_PendingPhysicalSError[liftState_simp]:
+  "\<lbrakk>write_reg PendingPhysicalSError_ref v\<rbrakk>\<^sub>S = updateS (regstate_update (PendingPhysicalSError_update (\<lambda>_. v)))"
   by (auto simp: liftState_write_reg_updateS register_defs)
 
-lemma liftS_read_reg_Sleeping[simp]:
-  "liftS (read_reg Sleeping_ref) = readS (Sleeping \<circ> regstate)"
+lemma liftS_read_reg_Sleeping[liftState_simp]:
+  "\<lbrakk>read_reg Sleeping_ref\<rbrakk>\<^sub>S = readS (Sleeping \<circ> regstate)"
   by (auto simp: liftState_read_reg_readS register_defs)
 
-lemma liftS_write_reg_Sleeping[simp]:
-  "liftS (write_reg Sleeping_ref v) = updateS (regstate_update (Sleeping_update (\<lambda>_. v)))"
+lemma liftS_write_reg_Sleeping[liftState_simp]:
+  "\<lbrakk>write_reg Sleeping_ref v\<rbrakk>\<^sub>S = updateS (regstate_update (Sleeping_update (\<lambda>_. v)))"
   by (auto simp: liftState_write_reg_updateS register_defs)
 
-lemma liftS_read_reg_ThisInstr[simp]:
-  "liftS (read_reg ThisInstr_ref) = readS (ThisInstr \<circ> regstate)"
+lemma liftS_read_reg_ThisInstr[liftState_simp]:
+  "\<lbrakk>read_reg ThisInstr_ref\<rbrakk>\<^sub>S = readS (ThisInstr \<circ> regstate)"
   by (auto simp: liftState_read_reg_readS register_defs)
 
-lemma liftS_write_reg_ThisInstr[simp]:
-  "liftS (write_reg ThisInstr_ref v) = updateS (regstate_update (ThisInstr_update (\<lambda>_. v)))"
+lemma liftS_write_reg_ThisInstr[liftState_simp]:
+  "\<lbrakk>write_reg ThisInstr_ref v\<rbrakk>\<^sub>S = updateS (regstate_update (ThisInstr_update (\<lambda>_. v)))"
   by (auto simp: liftState_write_reg_updateS register_defs)
 
-lemma liftS_read_reg_ThisInstrEnc[simp]:
-  "liftS (read_reg ThisInstrEnc_ref) = readS (ThisInstrEnc \<circ> regstate)"
+lemma liftS_read_reg_ThisInstrEnc[liftState_simp]:
+  "\<lbrakk>read_reg ThisInstrEnc_ref\<rbrakk>\<^sub>S = readS (ThisInstrEnc \<circ> regstate)"
   by (auto simp: liftState_read_reg_readS register_defs)
 
-lemma liftS_write_reg_ThisInstrEnc[simp]:
-  "liftS (write_reg ThisInstrEnc_ref v) = updateS (regstate_update (ThisInstrEnc_update (\<lambda>_. v)))"
+lemma liftS_write_reg_ThisInstrEnc[liftState_simp]:
+  "\<lbrakk>write_reg ThisInstrEnc_ref v\<rbrakk>\<^sub>S = updateS (regstate_update (ThisInstrEnc_update (\<lambda>_. v)))"
   by (auto simp: liftState_write_reg_updateS register_defs)
 
-lemma liftS_read_reg_currentCond[simp]:
-  "liftS (read_reg currentCond_ref) = readS (currentCond \<circ> regstate)"
+lemma liftS_read_reg_currentCond[liftState_simp]:
+  "\<lbrakk>read_reg currentCond_ref\<rbrakk>\<^sub>S = readS (currentCond \<circ> regstate)"
   by (auto simp: liftState_read_reg_readS register_defs)
 
-lemma liftS_write_reg_currentCond[simp]:
-  "liftS (write_reg currentCond_ref v) = updateS (regstate_update (currentCond_update (\<lambda>_. v)))"
+lemma liftS_write_reg_currentCond[liftState_simp]:
+  "\<lbrakk>write_reg currentCond_ref v\<rbrakk>\<^sub>S = updateS (regstate_update (currentCond_update (\<lambda>_. v)))"
   by (auto simp: liftState_write_reg_updateS register_defs)
 
-lemma liftS_read_reg_unconditional[simp]:
-  "liftS (read_reg unconditional_ref) = readS (unconditional \<circ> regstate)"
+lemma liftS_read_reg_unconditional[liftState_simp]:
+  "\<lbrakk>read_reg unconditional_ref\<rbrakk>\<^sub>S = readS (unconditional \<circ> regstate)"
   by (auto simp: liftState_read_reg_readS register_defs)
 
-lemma liftS_write_reg_unconditional[simp]:
-  "liftS (write_reg unconditional_ref v) = updateS (regstate_update (unconditional_update (\<lambda>_. v)))"
+lemma liftS_write_reg_unconditional[liftState_simp]:
+  "\<lbrakk>write_reg unconditional_ref v\<rbrakk>\<^sub>S = updateS (regstate_update (unconditional_update (\<lambda>_. v)))"
   by (auto simp: liftState_write_reg_updateS register_defs)
 
 end
